Milestone 5B.0: Capability-governed effect policy

internal/dafny_effect_reducer/EffectReducer.go
@@ -1,0 +1,2491 @@
+// Package EffectReducer
+// Dafny module EffectReducer compiled into Go
+
+package dafny_effect_reducer
+
+import (
+	m__System "github.com/dafny-lang/DafnyRuntimeGo/v4/System_"
+	_dafny "github.com/dafny-lang/DafnyRuntimeGo/v4/dafny"
+	os "os"
+)
+
+var _ = os.Args
+var _ _dafny.Dummy__
+var _ m__System.Dummy__
+
+type Dummy__ struct{}
+
+// Definition of class Default__
+type Default__ struct {
+	dummy byte
+}
+
+func New_Default___() *Default__ {
+	_this := Default__{}
+
+	return &_this
+}
+
+type CompanionStruct_Default___ struct {
+}
+
+var Companion_Default___ = CompanionStruct_Default___{}
+
+func (_this *Default__) Equals(other *Default__) bool {
+	return _this == other
+}
+
+func (_this *Default__) EqualsGeneric(x interface{}) bool {
+	other, ok := x.(*Default__)
+	return ok && _this.Equals(other)
+}
+
+func (*Default__) String() string {
+	return "_module.Default__"
+}
+func (_this *Default__) ParentTraits_() []*_dafny.TraitID {
+	return [](*_dafny.TraitID){}
+}
+
+var _ _dafny.TraitOffspring = &Default__{}
+
+func (_static *CompanionStruct_Default___) Decide(state EffectState, cmd Command) Decision {
+	var _source0 Command = cmd
+	_ = _source0
+	{
+		if _source0.Is_CommandClaimEffect() {
+			var _0_effectID _dafny.Sequence = _source0.Get_().(Command_CommandClaimEffect).EffectID
+			_ = _0_effectID
+			var _1_workerID _dafny.Sequence = _source0.Get_().(Command_CommandClaimEffect).WorkerID
+			_ = _1_workerID
+			var _2_expectedVersion _dafny.Int = _source0.Get_().(Command_CommandClaimEffect).ExpectedVersion
+			_ = _2_expectedVersion
+			var _3_leaseUntil _dafny.Int = _source0.Get_().(Command_CommandClaimEffect).LeaseUntil
+			_ = _3_leaseUntil
+			var _4_currentTime _dafny.Int = _source0.Get_().(Command_CommandClaimEffect).CurrentTime
+			_ = _4_currentTime
+			if (((state).Dtor_phase()).Equals(Companion_EffectPhase_.Create_SucceededPhase_())) || (((state).Dtor_phase()).Equals(Companion_EffectPhase_.Create_FailedTerminalPhase_())) {
+				return Companion_Decision_.Create_Decision_(Companion_DecisionStatus_.Create_Rejected_(), _dafny.SeqOf(Companion_Event_.Create_EventEffectRejected_(_0_effectID, _dafny.UnicodeSeqOfUtf8Bytes("effect already terminal"))))
+			} else if (((state).Dtor_phase()).Equals(Companion_EffectPhase_.Create_Claimed_())) && ((_4_currentTime).Cmp((state).Dtor_leaseUntil()) < 0) {
+				return Companion_Decision_.Create_Decision_(Companion_DecisionStatus_.Create_Rejected_(), _dafny.SeqOf(Companion_Event_.Create_EventEffectRejected_(_0_effectID, _dafny.UnicodeSeqOfUtf8Bytes("effect already claimed and unexpired"))))
+			} else if ((state).Dtor_retries()).Cmp(_dafny.IntOfInt64(3)) >= 0 {
+				return Companion_Decision_.Create_Decision_(Companion_DecisionStatus_.Create_Rejected_(), _dafny.SeqOf(Companion_Event_.Create_EventEffectTerminalized_(_0_effectID, _dafny.UnicodeSeqOfUtf8Bytes("retry limit reached"))))
+			} else {
+				return Companion_Decision_.Create_Decision_(Companion_DecisionStatus_.Create_Accepted_(), _dafny.SeqOf(Companion_Event_.Create_EventEffectClaimed_(_0_effectID, _1_workerID, ((state).Dtor_claimEpoch()).Plus(_dafny.One), _3_leaseUntil)))
+			}
+		}
+	}
+	{
+		if _source0.Is_CommandObserveEffect() {
+			var _5_effectID _dafny.Sequence = _source0.Get_().(Command_CommandObserveEffect).EffectID
+			_ = _5_effectID
+			var _6_workerID _dafny.Sequence = _source0.Get_().(Command_CommandObserveEffect).WorkerID
+			_ = _6_workerID
+			var _7_claimEpoch _dafny.Int = _source0.Get_().(Command_CommandObserveEffect).ClaimEpoch
+			_ = _7_claimEpoch
+			var _8_outcome Outcome = _source0.Get_().(Command_CommandObserveEffect).Outcome
+			_ = _8_outcome
+			if (_7_claimEpoch).Cmp((state).Dtor_claimEpoch()) < 0 {
+				return Companion_Decision_.Create_Decision_(Companion_DecisionStatus_.Create_Rejected_(), _dafny.SeqOf(Companion_Event_.Create_EventEffectRejected_(_5_effectID, _dafny.UnicodeSeqOfUtf8Bytes("stale claim epoch"))))
+			} else if !((state).Dtor_phase()).Equals(Companion_EffectPhase_.Create_Claimed_()) {
+				return Companion_Decision_.Create_Decision_(Companion_DecisionStatus_.Create_Rejected_(), _dafny.SeqOf(Companion_Event_.Create_EventEffectRejected_(_5_effectID, _dafny.UnicodeSeqOfUtf8Bytes("effect not claimed"))))
+			} else {
+				return Companion_Decision_.Create_Decision_(Companion_DecisionStatus_.Create_Accepted_(), _dafny.SeqOf(Companion_Event_.Create_EventEffectObserved_(_5_effectID, _7_claimEpoch, _8_outcome)))
+			}
+		}
+	}
+	{
+		if _source0.Is_CommandRetryEffect() {
+			var _9_effectID _dafny.Sequence = _source0.Get_().(Command_CommandRetryEffect).EffectID
+			_ = _9_effectID
+			if (((state).Dtor_phase()).Equals(Companion_EffectPhase_.Create_SucceededPhase_())) || (((state).Dtor_phase()).Equals(Companion_EffectPhase_.Create_FailedTerminalPhase_())) {
+				return Companion_Decision_.Create_Decision_(Companion_DecisionStatus_.Create_Rejected_(), _dafny.SeqOf(Companion_Event_.Create_EventEffectRejected_(_9_effectID, _dafny.UnicodeSeqOfUtf8Bytes("effect already terminal"))))
+			} else if (((state).Dtor_phase()).Equals(Companion_EffectPhase_.Create_FailedRetryablePhase_())) || (((state).Dtor_phase()).Equals(Companion_EffectPhase_.Create_OutcomeUnknownPhase_())) {
+				return Companion_Decision_.Create_Decision_(Companion_DecisionStatus_.Create_Accepted_(), _dafny.SeqOf(Companion_Event_.Create_EventEffectRetried_(_9_effectID)))
+			} else {
+				return Companion_Decision_.Create_Decision_(Companion_DecisionStatus_.Create_Rejected_(), _dafny.SeqOf(Companion_Event_.Create_EventEffectRejected_(_9_effectID, _dafny.UnicodeSeqOfUtf8Bytes("not in retryable state"))))
+			}
+		}
+	}
+	{
+		var _10_effectID _dafny.Sequence = _source0.Get_().(Command_CommandResolveUnknown).EffectID
+		_ = _10_effectID
+		var _11_caps CapabilityDescriptor = _source0.Get_().(Command_CommandResolveUnknown).Caps
+		_ = _11_caps
+		if !((state).Dtor_phase()).Equals(Companion_EffectPhase_.Create_OutcomeUnknownPhase_()) {
+			return Companion_Decision_.Create_Decision_(Companion_DecisionStatus_.Create_Rejected_(), _dafny.SeqOf(Companion_Event_.Create_EventEffectRejected_(_10_effectID, _dafny.UnicodeSeqOfUtf8Bytes("effect is not in unknown state"))))
+		} else if !((_11_caps).Dtor_status()).Equals(Companion_VerificationStatus_.Create_Verified_()) {
+			return Companion_Decision_.Create_Decision_(Companion_DecisionStatus_.Create_Accepted_(), _dafny.SeqOf(Companion_Event_.Create_EventManualResolutionRequired_(_10_effectID)))
+		} else if !((_11_caps).Dtor_resultLookup()).Equals(Companion_ResultLookupCapability_.Create_ResultLookupNone_()) {
+			return Companion_Decision_.Create_Decision_(Companion_DecisionStatus_.Create_Accepted_(), _dafny.SeqOf(Companion_Event_.Create_EventReconciliationRequired_(_10_effectID)))
+		} else if (!((_11_caps).Dtor_idempotency()).Equals(Companion_IdempotencyCapability_.Create_IdempotencyNone_())) && (((_11_caps).Dtor_unknownOutcome()).Equals(Companion_UnknownOutcomeCapability_.Create_CanSafelyRetry_())) {
+			return Companion_Decision_.Create_Decision_(Companion_DecisionStatus_.Create_Accepted_(), _dafny.SeqOf(Companion_Event_.Create_EventRetryAuthorized_(_10_effectID)))
+		} else {
+			return Companion_Decision_.Create_Decision_(Companion_DecisionStatus_.Create_Accepted_(), _dafny.SeqOf(Companion_Event_.Create_EventManualResolutionRequired_(_10_effectID)))
+		}
+	}
+}
+func (_static *CompanionStruct_Default___) Apply(state EffectState, event Event) EffectState {
+	var _source0 Event = event
+	_ = _source0
+	{
+		if _source0.Is_EventEffectClaimed() {
+			var _0_workerID _dafny.Sequence = _source0.Get_().(Event_EventEffectClaimed).WorkerID
+			_ = _0_workerID
+			var _1_claimEpoch _dafny.Int = _source0.Get_().(Event_EventEffectClaimed).ClaimEpoch
+			_ = _1_claimEpoch
+			var _2_leaseUntil _dafny.Int = _source0.Get_().(Event_EventEffectClaimed).LeaseUntil
+			_ = _2_leaseUntil
+			return Companion_EffectState_.Create_EffectState_((state).Dtor_effectID(), (state).Dtor_attemptID(), Companion_EffectPhase_.Create_Claimed_(), _0_workerID, _1_claimEpoch, _2_leaseUntil, ((state).Dtor_retries()).Plus(_dafny.One))
+		}
+	}
+	{
+		if _source0.Is_EventEffectObserved() {
+			var _3_outcome Outcome = _source0.Get_().(Event_EventEffectObserved).Outcome
+			_ = _3_outcome
+			var _4_newPhase EffectPhase = func() EffectPhase {
+				var _source1 Outcome = _3_outcome
+				_ = _source1
+				{
+					if _source1.Is_Succeeded() {
+						return Companion_EffectPhase_.Create_SucceededPhase_()
+					}
+				}
+				{
+					if _source1.Is_FailedRetryable() {
+						return Companion_EffectPhase_.Create_FailedRetryablePhase_()
+					}
+				}
+				{
+					if _source1.Is_FailedTerminal() {
+						return Companion_EffectPhase_.Create_FailedTerminalPhase_()
+					}
+				}
+				{
+					return Companion_EffectPhase_.Create_OutcomeUnknownPhase_()
+				}
+			}()
+			_ = _4_newPhase
+			return Companion_EffectState_.Create_EffectState_((state).Dtor_effectID(), (state).Dtor_attemptID(), _4_newPhase, (state).Dtor_workerID(), (state).Dtor_claimEpoch(), (state).Dtor_leaseUntil(), (state).Dtor_retries())
+		}
+	}
+	{
+		if _source0.Is_EventEffectRetried() {
+			return Companion_EffectState_.Create_EffectState_((state).Dtor_effectID(), (state).Dtor_attemptID(), Companion_EffectPhase_.Create_Pending_(), _dafny.UnicodeSeqOfUtf8Bytes(""), (state).Dtor_claimEpoch(), _dafny.Zero, (state).Dtor_retries())
+		}
+	}
+	{
+		if _source0.Is_EventEffectTerminalized() {
+			return Companion_EffectState_.Create_EffectState_((state).Dtor_effectID(), (state).Dtor_attemptID(), Companion_EffectPhase_.Create_FailedTerminalPhase_(), (state).Dtor_workerID(), (state).Dtor_claimEpoch(), (state).Dtor_leaseUntil(), (state).Dtor_retries())
+		}
+	}
+	{
+		if _source0.Is_EventEffectRejected() {
+			return state
+		}
+	}
+	{
+		if _source0.Is_EventManualResolutionRequired() {
+			return Companion_EffectState_.Create_EffectState_((state).Dtor_effectID(), (state).Dtor_attemptID(), Companion_EffectPhase_.Create_ManualResolutionRequiredPhase_(), (state).Dtor_workerID(), (state).Dtor_claimEpoch(), (state).Dtor_leaseUntil(), (state).Dtor_retries())
+		}
+	}
+	{
+		if _source0.Is_EventReconciliationRequired() {
+			return Companion_EffectState_.Create_EffectState_((state).Dtor_effectID(), (state).Dtor_attemptID(), Companion_EffectPhase_.Create_ReconciliationRequiredPhase_(), (state).Dtor_workerID(), (state).Dtor_claimEpoch(), (state).Dtor_leaseUntil(), (state).Dtor_retries())
+		}
+	}
+	{
+		return Companion_EffectState_.Create_EffectState_((state).Dtor_effectID(), (state).Dtor_attemptID(), Companion_EffectPhase_.Create_Pending_(), _dafny.UnicodeSeqOfUtf8Bytes(""), (state).Dtor_claimEpoch(), _dafny.Zero, (state).Dtor_retries())
+	}
+}
+func (_static *CompanionStruct_Default___) ApplyBatch(state EffectState, events _dafny.Sequence) EffectState {
+	goto TAIL_CALL_START
+TAIL_CALL_START:
+	if (_dafny.IntOfUint32((events).Cardinality())).Sign() == 0 {
+		return state
+	} else {
+		var _in0 EffectState = Companion_Default___.Apply(state, (events).Select(0).(Event))
+		_ = _in0
+		var _in1 _dafny.Sequence = (events).Drop(1)
+		_ = _in1
+		state = _in0
+		events = _in1
+		goto TAIL_CALL_START
+	}
+}
+
+// End of class Default__
+
+// Definition of datatype Outcome
+type Outcome struct {
+	Data_Outcome_
+}
+
+func (_this Outcome) Get_() Data_Outcome_ {
+	return _this.Data_Outcome_
+}
+
+type Data_Outcome_ interface {
+	isOutcome()
+}
+
+type CompanionStruct_Outcome_ struct {
+}
+
+var Companion_Outcome_ = CompanionStruct_Outcome_{}
+
+type Outcome_Succeeded struct {
+}
+
+func (Outcome_Succeeded) isOutcome() {}
+
+func (CompanionStruct_Outcome_) Create_Succeeded_() Outcome {
+	return Outcome{Outcome_Succeeded{}}
+}
+
+func (_this Outcome) Is_Succeeded() bool {
+	_, ok := _this.Get_().(Outcome_Succeeded)
+	return ok
+}
+
+type Outcome_FailedRetryable struct {
+}
+
+func (Outcome_FailedRetryable) isOutcome() {}
+
+func (CompanionStruct_Outcome_) Create_FailedRetryable_() Outcome {
+	return Outcome{Outcome_FailedRetryable{}}
+}
+
+func (_this Outcome) Is_FailedRetryable() bool {
+	_, ok := _this.Get_().(Outcome_FailedRetryable)
+	return ok
+}
+
+type Outcome_FailedTerminal struct {
+}
+
+func (Outcome_FailedTerminal) isOutcome() {}
+
+func (CompanionStruct_Outcome_) Create_FailedTerminal_() Outcome {
+	return Outcome{Outcome_FailedTerminal{}}
+}
+
+func (_this Outcome) Is_FailedTerminal() bool {
+	_, ok := _this.Get_().(Outcome_FailedTerminal)
+	return ok
+}
+
+type Outcome_OutcomeUnknown struct {
+}
+
+func (Outcome_OutcomeUnknown) isOutcome() {}
+
+func (CompanionStruct_Outcome_) Create_OutcomeUnknown_() Outcome {
+	return Outcome{Outcome_OutcomeUnknown{}}
+}
+
+func (_this Outcome) Is_OutcomeUnknown() bool {
+	_, ok := _this.Get_().(Outcome_OutcomeUnknown)
+	return ok
+}
+
+func (CompanionStruct_Outcome_) Default() Outcome {
+	return Companion_Outcome_.Create_Succeeded_()
+}
+
+func (_ CompanionStruct_Outcome_) AllSingletonConstructors() _dafny.Iterator {
+	i := -1
+	return func() (interface{}, bool) {
+		i++
+		switch i {
+		case 0:
+			return Companion_Outcome_.Create_Succeeded_(), true
+		case 1:
+			return Companion_Outcome_.Create_FailedRetryable_(), true
+		case 2:
+			return Companion_Outcome_.Create_FailedTerminal_(), true
+		case 3:
+			return Companion_Outcome_.Create_OutcomeUnknown_(), true
+		default:
+			return Outcome{}, false
+		}
+	}
+}
+
+func (_this Outcome) String() string {
+	switch _this.Get_().(type) {
+	case nil:
+		return "null"
+	case Outcome_Succeeded:
+		{
+			return "EffectReducer.Outcome.Succeeded"
+		}
+	case Outcome_FailedRetryable:
+		{
+			return "EffectReducer.Outcome.FailedRetryable"
+		}
+	case Outcome_FailedTerminal:
+		{
+			return "EffectReducer.Outcome.FailedTerminal"
+		}
+	case Outcome_OutcomeUnknown:
+		{
+			return "EffectReducer.Outcome.OutcomeUnknown"
+		}
+	default:
+		{
+			return "<unexpected>"
+		}
+	}
+}
+
+func (_this Outcome) Equals(other Outcome) bool {
+	switch _this.Get_().(type) {
+	case Outcome_Succeeded:
+		{
+			_, ok := other.Get_().(Outcome_Succeeded)
+			return ok
+		}
+	case Outcome_FailedRetryable:
+		{
+			_, ok := other.Get_().(Outcome_FailedRetryable)
+			return ok
+		}
+	case Outcome_FailedTerminal:
+		{
+			_, ok := other.Get_().(Outcome_FailedTerminal)
+			return ok
+		}
+	case Outcome_OutcomeUnknown:
+		{
+			_, ok := other.Get_().(Outcome_OutcomeUnknown)
+			return ok
+		}
+	default:
+		{
+			return false // unexpected
+		}
+	}
+}
+
+func (_this Outcome) EqualsGeneric(other interface{}) bool {
+	typed, ok := other.(Outcome)
+	return ok && _this.Equals(typed)
+}
+
+func Type_Outcome_() _dafny.TypeDescriptor {
+	return type_Outcome_{}
+}
+
+type type_Outcome_ struct {
+}
+
+func (_this type_Outcome_) Default() interface{} {
+	return Companion_Outcome_.Default()
+}
+
+func (_this type_Outcome_) String() string {
+	return "EffectReducer.Outcome"
+}
+func (_this Outcome) ParentTraits_() []*_dafny.TraitID {
+	return [](*_dafny.TraitID){}
+}
+
+var _ _dafny.TraitOffspring = Outcome{}
+
+// End of datatype Outcome
+
+// Definition of datatype EffectPhase
+type EffectPhase struct {
+	Data_EffectPhase_
+}
+
+func (_this EffectPhase) Get_() Data_EffectPhase_ {
+	return _this.Data_EffectPhase_
+}
+
+type Data_EffectPhase_ interface {
+	isEffectPhase()
+}
+
+type CompanionStruct_EffectPhase_ struct {
+}
+
+var Companion_EffectPhase_ = CompanionStruct_EffectPhase_{}
+
+type EffectPhase_Pending struct {
+}
+
+func (EffectPhase_Pending) isEffectPhase() {}
+
+func (CompanionStruct_EffectPhase_) Create_Pending_() EffectPhase {
+	return EffectPhase{EffectPhase_Pending{}}
+}
+
+func (_this EffectPhase) Is_Pending() bool {
+	_, ok := _this.Get_().(EffectPhase_Pending)
+	return ok
+}
+
+type EffectPhase_Claimed struct {
+}
+
+func (EffectPhase_Claimed) isEffectPhase() {}
+
+func (CompanionStruct_EffectPhase_) Create_Claimed_() EffectPhase {
+	return EffectPhase{EffectPhase_Claimed{}}
+}
+
+func (_this EffectPhase) Is_Claimed() bool {
+	_, ok := _this.Get_().(EffectPhase_Claimed)
+	return ok
+}
+
+type EffectPhase_SucceededPhase struct {
+}
+
+func (EffectPhase_SucceededPhase) isEffectPhase() {}
+
+func (CompanionStruct_EffectPhase_) Create_SucceededPhase_() EffectPhase {
+	return EffectPhase{EffectPhase_SucceededPhase{}}
+}
+
+func (_this EffectPhase) Is_SucceededPhase() bool {
+	_, ok := _this.Get_().(EffectPhase_SucceededPhase)
+	return ok
+}
+
+type EffectPhase_FailedRetryablePhase struct {
+}
+
+func (EffectPhase_FailedRetryablePhase) isEffectPhase() {}
+
+func (CompanionStruct_EffectPhase_) Create_FailedRetryablePhase_() EffectPhase {
+	return EffectPhase{EffectPhase_FailedRetryablePhase{}}
+}
+
+func (_this EffectPhase) Is_FailedRetryablePhase() bool {
+	_, ok := _this.Get_().(EffectPhase_FailedRetryablePhase)
+	return ok
+}
+
+type EffectPhase_FailedTerminalPhase struct {
+}
+
+func (EffectPhase_FailedTerminalPhase) isEffectPhase() {}
+
+func (CompanionStruct_EffectPhase_) Create_FailedTerminalPhase_() EffectPhase {
+	return EffectPhase{EffectPhase_FailedTerminalPhase{}}
+}
+
+func (_this EffectPhase) Is_FailedTerminalPhase() bool {
+	_, ok := _this.Get_().(EffectPhase_FailedTerminalPhase)
+	return ok
+}
+
+type EffectPhase_OutcomeUnknownPhase struct {
+}
+
+func (EffectPhase_OutcomeUnknownPhase) isEffectPhase() {}
+
+func (CompanionStruct_EffectPhase_) Create_OutcomeUnknownPhase_() EffectPhase {
+	return EffectPhase{EffectPhase_OutcomeUnknownPhase{}}
+}
+
+func (_this EffectPhase) Is_OutcomeUnknownPhase() bool {
+	_, ok := _this.Get_().(EffectPhase_OutcomeUnknownPhase)
+	return ok
+}
+
+type EffectPhase_ReconciliationRequiredPhase struct {
+}
+
+func (EffectPhase_ReconciliationRequiredPhase) isEffectPhase() {}
+
+func (CompanionStruct_EffectPhase_) Create_ReconciliationRequiredPhase_() EffectPhase {
+	return EffectPhase{EffectPhase_ReconciliationRequiredPhase{}}
+}
+
+func (_this EffectPhase) Is_ReconciliationRequiredPhase() bool {
+	_, ok := _this.Get_().(EffectPhase_ReconciliationRequiredPhase)
+	return ok
+}
+
+type EffectPhase_ManualResolutionRequiredPhase struct {
+}
+
+func (EffectPhase_ManualResolutionRequiredPhase) isEffectPhase() {}
+
+func (CompanionStruct_EffectPhase_) Create_ManualResolutionRequiredPhase_() EffectPhase {
+	return EffectPhase{EffectPhase_ManualResolutionRequiredPhase{}}
+}
+
+func (_this EffectPhase) Is_ManualResolutionRequiredPhase() bool {
+	_, ok := _this.Get_().(EffectPhase_ManualResolutionRequiredPhase)
+	return ok
+}
+
+func (CompanionStruct_EffectPhase_) Default() EffectPhase {
+	return Companion_EffectPhase_.Create_Pending_()
+}
+
+func (_ CompanionStruct_EffectPhase_) AllSingletonConstructors() _dafny.Iterator {
+	i := -1
+	return func() (interface{}, bool) {
+		i++
+		switch i {
+		case 0:
+			return Companion_EffectPhase_.Create_Pending_(), true
+		case 1:
+			return Companion_EffectPhase_.Create_Claimed_(), true
+		case 2:
+			return Companion_EffectPhase_.Create_SucceededPhase_(), true
+		case 3:
+			return Companion_EffectPhase_.Create_FailedRetryablePhase_(), true
+		case 4:
+			return Companion_EffectPhase_.Create_FailedTerminalPhase_(), true
+		case 5:
+			return Companion_EffectPhase_.Create_OutcomeUnknownPhase_(), true
+		case 6:
+			return Companion_EffectPhase_.Create_ReconciliationRequiredPhase_(), true
+		case 7:
+			return Companion_EffectPhase_.Create_ManualResolutionRequiredPhase_(), true
+		default:
+			return EffectPhase{}, false
+		}
+	}
+}
+
+func (_this EffectPhase) String() string {
+	switch _this.Get_().(type) {
+	case nil:
+		return "null"
+	case EffectPhase_Pending:
+		{
+			return "EffectReducer.EffectPhase.Pending"
+		}
+	case EffectPhase_Claimed:
+		{
+			return "EffectReducer.EffectPhase.Claimed"
+		}
+	case EffectPhase_SucceededPhase:
+		{
+			return "EffectReducer.EffectPhase.SucceededPhase"
+		}
+	case EffectPhase_FailedRetryablePhase:
+		{
+			return "EffectReducer.EffectPhase.FailedRetryablePhase"
+		}
+	case EffectPhase_FailedTerminalPhase:
+		{
+			return "EffectReducer.EffectPhase.FailedTerminalPhase"
+		}
+	case EffectPhase_OutcomeUnknownPhase:
+		{
+			return "EffectReducer.EffectPhase.OutcomeUnknownPhase"
+		}
+	case EffectPhase_ReconciliationRequiredPhase:
+		{
+			return "EffectReducer.EffectPhase.ReconciliationRequiredPhase"
+		}
+	case EffectPhase_ManualResolutionRequiredPhase:
+		{
+			return "EffectReducer.EffectPhase.ManualResolutionRequiredPhase"
+		}
+	default:
+		{
+			return "<unexpected>"
+		}
+	}
+}
+
+func (_this EffectPhase) Equals(other EffectPhase) bool {
+	switch _this.Get_().(type) {
+	case EffectPhase_Pending:
+		{
+			_, ok := other.Get_().(EffectPhase_Pending)
+			return ok
+		}
+	case EffectPhase_Claimed:
+		{
+			_, ok := other.Get_().(EffectPhase_Claimed)
+			return ok
+		}
+	case EffectPhase_SucceededPhase:
+		{
+			_, ok := other.Get_().(EffectPhase_SucceededPhase)
+			return ok
+		}
+	case EffectPhase_FailedRetryablePhase:
+		{
+			_, ok := other.Get_().(EffectPhase_FailedRetryablePhase)
+			return ok
+		}
+	case EffectPhase_FailedTerminalPhase:
+		{
+			_, ok := other.Get_().(EffectPhase_FailedTerminalPhase)
+			return ok
+		}
+	case EffectPhase_OutcomeUnknownPhase:
+		{
+			_, ok := other.Get_().(EffectPhase_OutcomeUnknownPhase)
+			return ok
+		}
+	case EffectPhase_ReconciliationRequiredPhase:
+		{
+			_, ok := other.Get_().(EffectPhase_ReconciliationRequiredPhase)
+			return ok
+		}
+	case EffectPhase_ManualResolutionRequiredPhase:
+		{
+			_, ok := other.Get_().(EffectPhase_ManualResolutionRequiredPhase)
+			return ok
+		}
+	default:
+		{
+			return false // unexpected
+		}
+	}
+}
+
+func (_this EffectPhase) EqualsGeneric(other interface{}) bool {
+	typed, ok := other.(EffectPhase)
+	return ok && _this.Equals(typed)
+}
+
+func Type_EffectPhase_() _dafny.TypeDescriptor {
+	return type_EffectPhase_{}
+}
+
+type type_EffectPhase_ struct {
+}
+
+func (_this type_EffectPhase_) Default() interface{} {
+	return Companion_EffectPhase_.Default()
+}
+
+func (_this type_EffectPhase_) String() string {
+	return "EffectReducer.EffectPhase"
+}
+func (_this EffectPhase) ParentTraits_() []*_dafny.TraitID {
+	return [](*_dafny.TraitID){}
+}
+
+var _ _dafny.TraitOffspring = EffectPhase{}
+
+// End of datatype EffectPhase
+
+// Definition of datatype IdempotencyCapability
+type IdempotencyCapability struct {
+	Data_IdempotencyCapability_
+}
+
+func (_this IdempotencyCapability) Get_() Data_IdempotencyCapability_ {
+	return _this.Data_IdempotencyCapability_
+}
+
+type Data_IdempotencyCapability_ interface {
+	isIdempotencyCapability()
+}
+
+type CompanionStruct_IdempotencyCapability_ struct {
+}
+
+var Companion_IdempotencyCapability_ = CompanionStruct_IdempotencyCapability_{}
+
+type IdempotencyCapability_IdempotencyNone struct {
+}
+
+func (IdempotencyCapability_IdempotencyNone) isIdempotencyCapability() {}
+
+func (CompanionStruct_IdempotencyCapability_) Create_IdempotencyNone_() IdempotencyCapability {
+	return IdempotencyCapability{IdempotencyCapability_IdempotencyNone{}}
+}
+
+func (_this IdempotencyCapability) Is_IdempotencyNone() bool {
+	_, ok := _this.Get_().(IdempotencyCapability_IdempotencyNone)
+	return ok
+}
+
+type IdempotencyCapability_StableKey struct {
+}
+
+func (IdempotencyCapability_StableKey) isIdempotencyCapability() {}
+
+func (CompanionStruct_IdempotencyCapability_) Create_StableKey_() IdempotencyCapability {
+	return IdempotencyCapability{IdempotencyCapability_StableKey{}}
+}
+
+func (_this IdempotencyCapability) Is_StableKey() bool {
+	_, ok := _this.Get_().(IdempotencyCapability_StableKey)
+	return ok
+}
+
+type IdempotencyCapability_StableKeyWithConflictDetection struct {
+}
+
+func (IdempotencyCapability_StableKeyWithConflictDetection) isIdempotencyCapability() {}
+
+func (CompanionStruct_IdempotencyCapability_) Create_StableKeyWithConflictDetection_() IdempotencyCapability {
+	return IdempotencyCapability{IdempotencyCapability_StableKeyWithConflictDetection{}}
+}
+
+func (_this IdempotencyCapability) Is_StableKeyWithConflictDetection() bool {
+	_, ok := _this.Get_().(IdempotencyCapability_StableKeyWithConflictDetection)
+	return ok
+}
+
+func (CompanionStruct_IdempotencyCapability_) Default() IdempotencyCapability {
+	return Companion_IdempotencyCapability_.Create_IdempotencyNone_()
+}
+
+func (_ CompanionStruct_IdempotencyCapability_) AllSingletonConstructors() _dafny.Iterator {
+	i := -1
+	return func() (interface{}, bool) {
+		i++
+		switch i {
+		case 0:
+			return Companion_IdempotencyCapability_.Create_IdempotencyNone_(), true
+		case 1:
+			return Companion_IdempotencyCapability_.Create_StableKey_(), true
+		case 2:
+			return Companion_IdempotencyCapability_.Create_StableKeyWithConflictDetection_(), true
+		default:
+			return IdempotencyCapability{}, false
+		}
+	}
+}
+
+func (_this IdempotencyCapability) String() string {
+	switch _this.Get_().(type) {
+	case nil:
+		return "null"
+	case IdempotencyCapability_IdempotencyNone:
+		{
+			return "EffectReducer.IdempotencyCapability.IdempotencyNone"
+		}
+	case IdempotencyCapability_StableKey:
+		{
+			return "EffectReducer.IdempotencyCapability.StableKey"
+		}
+	case IdempotencyCapability_StableKeyWithConflictDetection:
+		{
+			return "EffectReducer.IdempotencyCapability.StableKeyWithConflictDetection"
+		}
+	default:
+		{
+			return "<unexpected>"
+		}
+	}
+}
+
+func (_this IdempotencyCapability) Equals(other IdempotencyCapability) bool {
+	switch _this.Get_().(type) {
+	case IdempotencyCapability_IdempotencyNone:
+		{
+			_, ok := other.Get_().(IdempotencyCapability_IdempotencyNone)
+			return ok
+		}
+	case IdempotencyCapability_StableKey:
+		{
+			_, ok := other.Get_().(IdempotencyCapability_StableKey)
+			return ok
+		}
+	case IdempotencyCapability_StableKeyWithConflictDetection:
+		{
+			_, ok := other.Get_().(IdempotencyCapability_StableKeyWithConflictDetection)
+			return ok
+		}
+	default:
+		{
+			return false // unexpected
+		}
+	}
+}
+
+func (_this IdempotencyCapability) EqualsGeneric(other interface{}) bool {
+	typed, ok := other.(IdempotencyCapability)
+	return ok && _this.Equals(typed)
+}
+
+func Type_IdempotencyCapability_() _dafny.TypeDescriptor {
+	return type_IdempotencyCapability_{}
+}
+
+type type_IdempotencyCapability_ struct {
+}
+
+func (_this type_IdempotencyCapability_) Default() interface{} {
+	return Companion_IdempotencyCapability_.Default()
+}
+
+func (_this type_IdempotencyCapability_) String() string {
+	return "EffectReducer.IdempotencyCapability"
+}
+func (_this IdempotencyCapability) ParentTraits_() []*_dafny.TraitID {
+	return [](*_dafny.TraitID){}
+}
+
+var _ _dafny.TraitOffspring = IdempotencyCapability{}
+
+// End of datatype IdempotencyCapability
+
+// Definition of datatype ResultLookupCapability
+type ResultLookupCapability struct {
+	Data_ResultLookupCapability_
+}
+
+func (_this ResultLookupCapability) Get_() Data_ResultLookupCapability_ {
+	return _this.Data_ResultLookupCapability_
+}
+
+type Data_ResultLookupCapability_ interface {
+	isResultLookupCapability()
+}
+
+type CompanionStruct_ResultLookupCapability_ struct {
+}
+
+var Companion_ResultLookupCapability_ = CompanionStruct_ResultLookupCapability_{}
+
+type ResultLookupCapability_ResultLookupNone struct {
+}
+
+func (ResultLookupCapability_ResultLookupNone) isResultLookupCapability() {}
+
+func (CompanionStruct_ResultLookupCapability_) Create_ResultLookupNone_() ResultLookupCapability {
+	return ResultLookupCapability{ResultLookupCapability_ResultLookupNone{}}
+}
+
+func (_this ResultLookupCapability) Is_ResultLookupNone() bool {
+	_, ok := _this.Get_().(ResultLookupCapability_ResultLookupNone)
+	return ok
+}
+
+type ResultLookupCapability_ByExternalReference struct {
+}
+
+func (ResultLookupCapability_ByExternalReference) isResultLookupCapability() {}
+
+func (CompanionStruct_ResultLookupCapability_) Create_ByExternalReference_() ResultLookupCapability {
+	return ResultLookupCapability{ResultLookupCapability_ByExternalReference{}}
+}
+
+func (_this ResultLookupCapability) Is_ByExternalReference() bool {
+	_, ok := _this.Get_().(ResultLookupCapability_ByExternalReference)
+	return ok
+}
+
+type ResultLookupCapability_ByIdempotencyKey struct {
+}
+
+func (ResultLookupCapability_ByIdempotencyKey) isResultLookupCapability() {}
+
+func (CompanionStruct_ResultLookupCapability_) Create_ByIdempotencyKey_() ResultLookupCapability {
+	return ResultLookupCapability{ResultLookupCapability_ByIdempotencyKey{}}
+}
+
+func (_this ResultLookupCapability) Is_ByIdempotencyKey() bool {
+	_, ok := _this.Get_().(ResultLookupCapability_ByIdempotencyKey)
+	return ok
+}
+
+func (CompanionStruct_ResultLookupCapability_) Default() ResultLookupCapability {
+	return Companion_ResultLookupCapability_.Create_ResultLookupNone_()
+}
+
+func (_ CompanionStruct_ResultLookupCapability_) AllSingletonConstructors() _dafny.Iterator {
+	i := -1
+	return func() (interface{}, bool) {
+		i++
+		switch i {
+		case 0:
+			return Companion_ResultLookupCapability_.Create_ResultLookupNone_(), true
+		case 1:
+			return Companion_ResultLookupCapability_.Create_ByExternalReference_(), true
+		case 2:
+			return Companion_ResultLookupCapability_.Create_ByIdempotencyKey_(), true
+		default:
+			return ResultLookupCapability{}, false
+		}
+	}
+}
+
+func (_this ResultLookupCapability) String() string {
+	switch _this.Get_().(type) {
+	case nil:
+		return "null"
+	case ResultLookupCapability_ResultLookupNone:
+		{
+			return "EffectReducer.ResultLookupCapability.ResultLookupNone"
+		}
+	case ResultLookupCapability_ByExternalReference:
+		{
+			return "EffectReducer.ResultLookupCapability.ByExternalReference"
+		}
+	case ResultLookupCapability_ByIdempotencyKey:
+		{
+			return "EffectReducer.ResultLookupCapability.ByIdempotencyKey"
+		}
+	default:
+		{
+			return "<unexpected>"
+		}
+	}
+}
+
+func (_this ResultLookupCapability) Equals(other ResultLookupCapability) bool {
+	switch _this.Get_().(type) {
+	case ResultLookupCapability_ResultLookupNone:
+		{
+			_, ok := other.Get_().(ResultLookupCapability_ResultLookupNone)
+			return ok
+		}
+	case ResultLookupCapability_ByExternalReference:
+		{
+			_, ok := other.Get_().(ResultLookupCapability_ByExternalReference)
+			return ok
+		}
+	case ResultLookupCapability_ByIdempotencyKey:
+		{
+			_, ok := other.Get_().(ResultLookupCapability_ByIdempotencyKey)
+			return ok
+		}
+	default:
+		{
+			return false // unexpected
+		}
+	}
+}
+
+func (_this ResultLookupCapability) EqualsGeneric(other interface{}) bool {
+	typed, ok := other.(ResultLookupCapability)
+	return ok && _this.Equals(typed)
+}
+
+func Type_ResultLookupCapability_() _dafny.TypeDescriptor {
+	return type_ResultLookupCapability_{}
+}
+
+type type_ResultLookupCapability_ struct {
+}
+
+func (_this type_ResultLookupCapability_) Default() interface{} {
+	return Companion_ResultLookupCapability_.Default()
+}
+
+func (_this type_ResultLookupCapability_) String() string {
+	return "EffectReducer.ResultLookupCapability"
+}
+func (_this ResultLookupCapability) ParentTraits_() []*_dafny.TraitID {
+	return [](*_dafny.TraitID){}
+}
+
+var _ _dafny.TraitOffspring = ResultLookupCapability{}
+
+// End of datatype ResultLookupCapability
+
+// Definition of datatype TransactionCapability
+type TransactionCapability struct {
+	Data_TransactionCapability_
+}
+
+func (_this TransactionCapability) Get_() Data_TransactionCapability_ {
+	return _this.Data_TransactionCapability_
+}
+
+type Data_TransactionCapability_ interface {
+	isTransactionCapability()
+}
+
+type CompanionStruct_TransactionCapability_ struct {
+}
+
+var Companion_TransactionCapability_ = CompanionStruct_TransactionCapability_{}
+
+type TransactionCapability_TransactionNone struct {
+}
+
+func (TransactionCapability_TransactionNone) isTransactionCapability() {}
+
+func (CompanionStruct_TransactionCapability_) Create_TransactionNone_() TransactionCapability {
+	return TransactionCapability{TransactionCapability_TransactionNone{}}
+}
+
+func (_this TransactionCapability) Is_TransactionNone() bool {
+	_, ok := _this.Get_().(TransactionCapability_TransactionNone)
+	return ok
+}
+
+type TransactionCapability_SingleOperation struct {
+}
+
+func (TransactionCapability_SingleOperation) isTransactionCapability() {}
+
+func (CompanionStruct_TransactionCapability_) Create_SingleOperation_() TransactionCapability {
+	return TransactionCapability{TransactionCapability_SingleOperation{}}
+}
+
+func (_this TransactionCapability) Is_SingleOperation() bool {
+	_, ok := _this.Get_().(TransactionCapability_SingleOperation)
+	return ok
+}
+
+type TransactionCapability_AtomicBatch struct {
+}
+
+func (TransactionCapability_AtomicBatch) isTransactionCapability() {}
+
+func (CompanionStruct_TransactionCapability_) Create_AtomicBatch_() TransactionCapability {
+	return TransactionCapability{TransactionCapability_AtomicBatch{}}
+}
+
+func (_this TransactionCapability) Is_AtomicBatch() bool {
+	_, ok := _this.Get_().(TransactionCapability_AtomicBatch)
+	return ok
+}
+
+func (CompanionStruct_TransactionCapability_) Default() TransactionCapability {
+	return Companion_TransactionCapability_.Create_TransactionNone_()
+}
+
+func (_ CompanionStruct_TransactionCapability_) AllSingletonConstructors() _dafny.Iterator {
+	i := -1
+	return func() (interface{}, bool) {
+		i++
+		switch i {
+		case 0:
+			return Companion_TransactionCapability_.Create_TransactionNone_(), true
+		case 1:
+			return Companion_TransactionCapability_.Create_SingleOperation_(), true
+		case 2:
+			return Companion_TransactionCapability_.Create_AtomicBatch_(), true
+		default:
+			return TransactionCapability{}, false
+		}
+	}
+}
+
+func (_this TransactionCapability) String() string {
+	switch _this.Get_().(type) {
+	case nil:
+		return "null"
+	case TransactionCapability_TransactionNone:
+		{
+			return "EffectReducer.TransactionCapability.TransactionNone"
+		}
+	case TransactionCapability_SingleOperation:
+		{
+			return "EffectReducer.TransactionCapability.SingleOperation"
+		}
+	case TransactionCapability_AtomicBatch:
+		{
+			return "EffectReducer.TransactionCapability.AtomicBatch"
+		}
+	default:
+		{
+			return "<unexpected>"
+		}
+	}
+}
+
+func (_this TransactionCapability) Equals(other TransactionCapability) bool {
+	switch _this.Get_().(type) {
+	case TransactionCapability_TransactionNone:
+		{
+			_, ok := other.Get_().(TransactionCapability_TransactionNone)
+			return ok
+		}
+	case TransactionCapability_SingleOperation:
+		{
+			_, ok := other.Get_().(TransactionCapability_SingleOperation)
+			return ok
+		}
+	case TransactionCapability_AtomicBatch:
+		{
+			_, ok := other.Get_().(TransactionCapability_AtomicBatch)
+			return ok
+		}
+	default:
+		{
+			return false // unexpected
+		}
+	}
+}
+
+func (_this TransactionCapability) EqualsGeneric(other interface{}) bool {
+	typed, ok := other.(TransactionCapability)
+	return ok && _this.Equals(typed)
+}
+
+func Type_TransactionCapability_() _dafny.TypeDescriptor {
+	return type_TransactionCapability_{}
+}
+
+type type_TransactionCapability_ struct {
+}
+
+func (_this type_TransactionCapability_) Default() interface{} {
+	return Companion_TransactionCapability_.Default()
+}
+
+func (_this type_TransactionCapability_) String() string {
+	return "EffectReducer.TransactionCapability"
+}
+func (_this TransactionCapability) ParentTraits_() []*_dafny.TraitID {
+	return [](*_dafny.TraitID){}
+}
+
+var _ _dafny.TraitOffspring = TransactionCapability{}
+
+// End of datatype TransactionCapability
+
+// Definition of datatype UnknownOutcomeCapability
+type UnknownOutcomeCapability struct {
+	Data_UnknownOutcomeCapability_
+}
+
+func (_this UnknownOutcomeCapability) Get_() Data_UnknownOutcomeCapability_ {
+	return _this.Data_UnknownOutcomeCapability_
+}
+
+type Data_UnknownOutcomeCapability_ interface {
+	isUnknownOutcomeCapability()
+}
+
+type CompanionStruct_UnknownOutcomeCapability_ struct {
+}
+
+var Companion_UnknownOutcomeCapability_ = CompanionStruct_UnknownOutcomeCapability_{}
+
+type UnknownOutcomeCapability_RequiresManualResolution struct {
+}
+
+func (UnknownOutcomeCapability_RequiresManualResolution) isUnknownOutcomeCapability() {}
+
+func (CompanionStruct_UnknownOutcomeCapability_) Create_RequiresManualResolution_() UnknownOutcomeCapability {
+	return UnknownOutcomeCapability{UnknownOutcomeCapability_RequiresManualResolution{}}
+}
+
+func (_this UnknownOutcomeCapability) Is_RequiresManualResolution() bool {
+	_, ok := _this.Get_().(UnknownOutcomeCapability_RequiresManualResolution)
+	return ok
+}
+
+type UnknownOutcomeCapability_CanReconcile struct {
+}
+
+func (UnknownOutcomeCapability_CanReconcile) isUnknownOutcomeCapability() {}
+
+func (CompanionStruct_UnknownOutcomeCapability_) Create_CanReconcile_() UnknownOutcomeCapability {
+	return UnknownOutcomeCapability{UnknownOutcomeCapability_CanReconcile{}}
+}
+
+func (_this UnknownOutcomeCapability) Is_CanReconcile() bool {
+	_, ok := _this.Get_().(UnknownOutcomeCapability_CanReconcile)
+	return ok
+}
+
+type UnknownOutcomeCapability_CanSafelyRetry struct {
+}
+
+func (UnknownOutcomeCapability_CanSafelyRetry) isUnknownOutcomeCapability() {}
+
+func (CompanionStruct_UnknownOutcomeCapability_) Create_CanSafelyRetry_() UnknownOutcomeCapability {
+	return UnknownOutcomeCapability{UnknownOutcomeCapability_CanSafelyRetry{}}
+}
+
+func (_this UnknownOutcomeCapability) Is_CanSafelyRetry() bool {
+	_, ok := _this.Get_().(UnknownOutcomeCapability_CanSafelyRetry)
+	return ok
+}
+
+func (CompanionStruct_UnknownOutcomeCapability_) Default() UnknownOutcomeCapability {
+	return Companion_UnknownOutcomeCapability_.Create_RequiresManualResolution_()
+}
+
+func (_ CompanionStruct_UnknownOutcomeCapability_) AllSingletonConstructors() _dafny.Iterator {
+	i := -1
+	return func() (interface{}, bool) {
+		i++
+		switch i {
+		case 0:
+			return Companion_UnknownOutcomeCapability_.Create_RequiresManualResolution_(), true
+		case 1:
+			return Companion_UnknownOutcomeCapability_.Create_CanReconcile_(), true
+		case 2:
+			return Companion_UnknownOutcomeCapability_.Create_CanSafelyRetry_(), true
+		default:
+			return UnknownOutcomeCapability{}, false
+		}
+	}
+}
+
+func (_this UnknownOutcomeCapability) String() string {
+	switch _this.Get_().(type) {
+	case nil:
+		return "null"
+	case UnknownOutcomeCapability_RequiresManualResolution:
+		{
+			return "EffectReducer.UnknownOutcomeCapability.RequiresManualResolution"
+		}
+	case UnknownOutcomeCapability_CanReconcile:
+		{
+			return "EffectReducer.UnknownOutcomeCapability.CanReconcile"
+		}
+	case UnknownOutcomeCapability_CanSafelyRetry:
+		{
+			return "EffectReducer.UnknownOutcomeCapability.CanSafelyRetry"
+		}
+	default:
+		{
+			return "<unexpected>"
+		}
+	}
+}
+
+func (_this UnknownOutcomeCapability) Equals(other UnknownOutcomeCapability) bool {
+	switch _this.Get_().(type) {
+	case UnknownOutcomeCapability_RequiresManualResolution:
+		{
+			_, ok := other.Get_().(UnknownOutcomeCapability_RequiresManualResolution)
+			return ok
+		}
+	case UnknownOutcomeCapability_CanReconcile:
+		{
+			_, ok := other.Get_().(UnknownOutcomeCapability_CanReconcile)
+			return ok
+		}
+	case UnknownOutcomeCapability_CanSafelyRetry:
+		{
+			_, ok := other.Get_().(UnknownOutcomeCapability_CanSafelyRetry)
+			return ok
+		}
+	default:
+		{
+			return false // unexpected
+		}
+	}
+}
+
+func (_this UnknownOutcomeCapability) EqualsGeneric(other interface{}) bool {
+	typed, ok := other.(UnknownOutcomeCapability)
+	return ok && _this.Equals(typed)
+}
+
+func Type_UnknownOutcomeCapability_() _dafny.TypeDescriptor {
+	return type_UnknownOutcomeCapability_{}
+}
+
+type type_UnknownOutcomeCapability_ struct {
+}
+
+func (_this type_UnknownOutcomeCapability_) Default() interface{} {
+	return Companion_UnknownOutcomeCapability_.Default()
+}
+
+func (_this type_UnknownOutcomeCapability_) String() string {
+	return "EffectReducer.UnknownOutcomeCapability"
+}
+func (_this UnknownOutcomeCapability) ParentTraits_() []*_dafny.TraitID {
+	return [](*_dafny.TraitID){}
+}
+
+var _ _dafny.TraitOffspring = UnknownOutcomeCapability{}
+
+// End of datatype UnknownOutcomeCapability
+
+// Definition of datatype VerificationStatus
+type VerificationStatus struct {
+	Data_VerificationStatus_
+}
+
+func (_this VerificationStatus) Get_() Data_VerificationStatus_ {
+	return _this.Data_VerificationStatus_
+}
+
+type Data_VerificationStatus_ interface {
+	isVerificationStatus()
+}
+
+type CompanionStruct_VerificationStatus_ struct {
+}
+
+var Companion_VerificationStatus_ = CompanionStruct_VerificationStatus_{}
+
+type VerificationStatus_Proposed struct {
+}
+
+func (VerificationStatus_Proposed) isVerificationStatus() {}
+
+func (CompanionStruct_VerificationStatus_) Create_Proposed_() VerificationStatus {
+	return VerificationStatus{VerificationStatus_Proposed{}}
+}
+
+func (_this VerificationStatus) Is_Proposed() bool {
+	_, ok := _this.Get_().(VerificationStatus_Proposed)
+	return ok
+}
+
+type VerificationStatus_Verified struct {
+}
+
+func (VerificationStatus_Verified) isVerificationStatus() {}
+
+func (CompanionStruct_VerificationStatus_) Create_Verified_() VerificationStatus {
+	return VerificationStatus{VerificationStatus_Verified{}}
+}
+
+func (_this VerificationStatus) Is_Verified() bool {
+	_, ok := _this.Get_().(VerificationStatus_Verified)
+	return ok
+}
+
+type VerificationStatus_Invalidated struct {
+}
+
+func (VerificationStatus_Invalidated) isVerificationStatus() {}
+
+func (CompanionStruct_VerificationStatus_) Create_Invalidated_() VerificationStatus {
+	return VerificationStatus{VerificationStatus_Invalidated{}}
+}
+
+func (_this VerificationStatus) Is_Invalidated() bool {
+	_, ok := _this.Get_().(VerificationStatus_Invalidated)
+	return ok
+}
+
+func (CompanionStruct_VerificationStatus_) Default() VerificationStatus {
+	return Companion_VerificationStatus_.Create_Proposed_()
+}
+
+func (_ CompanionStruct_VerificationStatus_) AllSingletonConstructors() _dafny.Iterator {
+	i := -1
+	return func() (interface{}, bool) {
+		i++
+		switch i {
+		case 0:
+			return Companion_VerificationStatus_.Create_Proposed_(), true
+		case 1:
+			return Companion_VerificationStatus_.Create_Verified_(), true
+		case 2:
+			return Companion_VerificationStatus_.Create_Invalidated_(), true
+		default:
+			return VerificationStatus{}, false
+		}
+	}
+}
+
+func (_this VerificationStatus) String() string {
+	switch _this.Get_().(type) {
+	case nil:
+		return "null"
+	case VerificationStatus_Proposed:
+		{
+			return "EffectReducer.VerificationStatus.Proposed"
+		}
+	case VerificationStatus_Verified:
+		{
+			return "EffectReducer.VerificationStatus.Verified"
+		}
+	case VerificationStatus_Invalidated:
+		{
+			return "EffectReducer.VerificationStatus.Invalidated"
+		}
+	default:
+		{
+			return "<unexpected>"
+		}
+	}
+}
+
+func (_this VerificationStatus) Equals(other VerificationStatus) bool {
+	switch _this.Get_().(type) {
+	case VerificationStatus_Proposed:
+		{
+			_, ok := other.Get_().(VerificationStatus_Proposed)
+			return ok
+		}
+	case VerificationStatus_Verified:
+		{
+			_, ok := other.Get_().(VerificationStatus_Verified)
+			return ok
+		}
+	case VerificationStatus_Invalidated:
+		{
+			_, ok := other.Get_().(VerificationStatus_Invalidated)
+			return ok
+		}
+	default:
+		{
+			return false // unexpected
+		}
+	}
+}
+
+func (_this VerificationStatus) EqualsGeneric(other interface{}) bool {
+	typed, ok := other.(VerificationStatus)
+	return ok && _this.Equals(typed)
+}
+
+func Type_VerificationStatus_() _dafny.TypeDescriptor {
+	return type_VerificationStatus_{}
+}
+
+type type_VerificationStatus_ struct {
+}
+
+func (_this type_VerificationStatus_) Default() interface{} {
+	return Companion_VerificationStatus_.Default()
+}
+
+func (_this type_VerificationStatus_) String() string {
+	return "EffectReducer.VerificationStatus"
+}
+func (_this VerificationStatus) ParentTraits_() []*_dafny.TraitID {
+	return [](*_dafny.TraitID){}
+}
+
+var _ _dafny.TraitOffspring = VerificationStatus{}
+
+// End of datatype VerificationStatus
+
+// Definition of datatype CapabilityDescriptor
+type CapabilityDescriptor struct {
+	Data_CapabilityDescriptor_
+}
+
+func (_this CapabilityDescriptor) Get_() Data_CapabilityDescriptor_ {
+	return _this.Data_CapabilityDescriptor_
+}
+
+type Data_CapabilityDescriptor_ interface {
+	isCapabilityDescriptor()
+}
+
+type CompanionStruct_CapabilityDescriptor_ struct {
+}
+
+var Companion_CapabilityDescriptor_ = CompanionStruct_CapabilityDescriptor_{}
+
+type CapabilityDescriptor_CapabilityDescriptor struct {
+	Idempotency      IdempotencyCapability
+	ResultLookup     ResultLookupCapability
+	Transactionality TransactionCapability
+	UnknownOutcome   UnknownOutcomeCapability
+	Status           VerificationStatus
+}
+
+func (CapabilityDescriptor_CapabilityDescriptor) isCapabilityDescriptor() {}
+
+func (CompanionStruct_CapabilityDescriptor_) Create_CapabilityDescriptor_(Idempotency IdempotencyCapability, ResultLookup ResultLookupCapability, Transactionality TransactionCapability, UnknownOutcome UnknownOutcomeCapability, Status VerificationStatus) CapabilityDescriptor {
+	return CapabilityDescriptor{CapabilityDescriptor_CapabilityDescriptor{Idempotency, ResultLookup, Transactionality, UnknownOutcome, Status}}
+}
+
+func (_this CapabilityDescriptor) Is_CapabilityDescriptor() bool {
+	_, ok := _this.Get_().(CapabilityDescriptor_CapabilityDescriptor)
+	return ok
+}
+
+func (CompanionStruct_CapabilityDescriptor_) Default() CapabilityDescriptor {
+	return Companion_CapabilityDescriptor_.Create_CapabilityDescriptor_(Companion_IdempotencyCapability_.Default(), Companion_ResultLookupCapability_.Default(), Companion_TransactionCapability_.Default(), Companion_UnknownOutcomeCapability_.Default(), Companion_VerificationStatus_.Default())
+}
+
+func (_this CapabilityDescriptor) Dtor_idempotency() IdempotencyCapability {
+	return _this.Get_().(CapabilityDescriptor_CapabilityDescriptor).Idempotency
+}
+
+func (_this CapabilityDescriptor) Dtor_resultLookup() ResultLookupCapability {
+	return _this.Get_().(CapabilityDescriptor_CapabilityDescriptor).ResultLookup
+}
+
+func (_this CapabilityDescriptor) Dtor_transactionality() TransactionCapability {
+	return _this.Get_().(CapabilityDescriptor_CapabilityDescriptor).Transactionality
+}
+
+func (_this CapabilityDescriptor) Dtor_unknownOutcome() UnknownOutcomeCapability {
+	return _this.Get_().(CapabilityDescriptor_CapabilityDescriptor).UnknownOutcome
+}
+
+func (_this CapabilityDescriptor) Dtor_status() VerificationStatus {
+	return _this.Get_().(CapabilityDescriptor_CapabilityDescriptor).Status
+}
+
+func (_this CapabilityDescriptor) String() string {
+	switch data := _this.Get_().(type) {
+	case nil:
+		return "null"
+	case CapabilityDescriptor_CapabilityDescriptor:
+		{
+			return "EffectReducer.CapabilityDescriptor.CapabilityDescriptor" + "(" + _dafny.String(data.Idempotency) + ", " + _dafny.String(data.ResultLookup) + ", " + _dafny.String(data.Transactionality) + ", " + _dafny.String(data.UnknownOutcome) + ", " + _dafny.String(data.Status) + ")"
+		}
+	default:
+		{
+			return "<unexpected>"
+		}
+	}
+}
+
+func (_this CapabilityDescriptor) Equals(other CapabilityDescriptor) bool {
+	switch data1 := _this.Get_().(type) {
+	case CapabilityDescriptor_CapabilityDescriptor:
+		{
+			data2, ok := other.Get_().(CapabilityDescriptor_CapabilityDescriptor)
+			return ok && data1.Idempotency.Equals(data2.Idempotency) && data1.ResultLookup.Equals(data2.ResultLookup) && data1.Transactionality.Equals(data2.Transactionality) && data1.UnknownOutcome.Equals(data2.UnknownOutcome) && data1.Status.Equals(data2.Status)
+		}
+	default:
+		{
+			return false // unexpected
+		}
+	}
+}
+
+func (_this CapabilityDescriptor) EqualsGeneric(other interface{}) bool {
+	typed, ok := other.(CapabilityDescriptor)
+	return ok && _this.Equals(typed)
+}
+
+func Type_CapabilityDescriptor_() _dafny.TypeDescriptor {
+	return type_CapabilityDescriptor_{}
+}
+
+type type_CapabilityDescriptor_ struct {
+}
+
+func (_this type_CapabilityDescriptor_) Default() interface{} {
+	return Companion_CapabilityDescriptor_.Default()
+}
+
+func (_this type_CapabilityDescriptor_) String() string {
+	return "EffectReducer.CapabilityDescriptor"
+}
+func (_this CapabilityDescriptor) ParentTraits_() []*_dafny.TraitID {
+	return [](*_dafny.TraitID){}
+}
+
+var _ _dafny.TraitOffspring = CapabilityDescriptor{}
+
+// End of datatype CapabilityDescriptor
+
+// Definition of datatype EffectState
+type EffectState struct {
+	Data_EffectState_
+}
+
+func (_this EffectState) Get_() Data_EffectState_ {
+	return _this.Data_EffectState_
+}
+
+type Data_EffectState_ interface {
+	isEffectState()
+}
+
+type CompanionStruct_EffectState_ struct {
+}
+
+var Companion_EffectState_ = CompanionStruct_EffectState_{}
+
+type EffectState_EffectState struct {
+	EffectID   _dafny.Sequence
+	AttemptID  _dafny.Sequence
+	Phase      EffectPhase
+	WorkerID   _dafny.Sequence
+	ClaimEpoch _dafny.Int
+	LeaseUntil _dafny.Int
+	Retries    _dafny.Int
+}
+
+func (EffectState_EffectState) isEffectState() {}
+
+func (CompanionStruct_EffectState_) Create_EffectState_(EffectID _dafny.Sequence, AttemptID _dafny.Sequence, Phase EffectPhase, WorkerID _dafny.Sequence, ClaimEpoch _dafny.Int, LeaseUntil _dafny.Int, Retries _dafny.Int) EffectState {
+	return EffectState{EffectState_EffectState{EffectID, AttemptID, Phase, WorkerID, ClaimEpoch, LeaseUntil, Retries}}
+}
+
+func (_this EffectState) Is_EffectState() bool {
+	_, ok := _this.Get_().(EffectState_EffectState)
+	return ok
+}
+
+func (CompanionStruct_EffectState_) Default() EffectState {
+	return Companion_EffectState_.Create_EffectState_(_dafny.EmptySeq, _dafny.EmptySeq, Companion_EffectPhase_.Default(), _dafny.EmptySeq, _dafny.Zero, _dafny.Zero, _dafny.Zero)
+}
+
+func (_this EffectState) Dtor_effectID() _dafny.Sequence {
+	return _this.Get_().(EffectState_EffectState).EffectID
+}
+
+func (_this EffectState) Dtor_attemptID() _dafny.Sequence {
+	return _this.Get_().(EffectState_EffectState).AttemptID
+}
+
+func (_this EffectState) Dtor_phase() EffectPhase {
+	return _this.Get_().(EffectState_EffectState).Phase
+}
+
+func (_this EffectState) Dtor_workerID() _dafny.Sequence {
+	return _this.Get_().(EffectState_EffectState).WorkerID
+}
+
+func (_this EffectState) Dtor_claimEpoch() _dafny.Int {
+	return _this.Get_().(EffectState_EffectState).ClaimEpoch
+}
+
+func (_this EffectState) Dtor_leaseUntil() _dafny.Int {
+	return _this.Get_().(EffectState_EffectState).LeaseUntil
+}
+
+func (_this EffectState) Dtor_retries() _dafny.Int {
+	return _this.Get_().(EffectState_EffectState).Retries
+}
+
+func (_this EffectState) String() string {
+	switch data := _this.Get_().(type) {
+	case nil:
+		return "null"
+	case EffectState_EffectState:
+		{
+			return "EffectReducer.EffectState.EffectState" + "(" + data.EffectID.VerbatimString(true) + ", " + data.AttemptID.VerbatimString(true) + ", " + _dafny.String(data.Phase) + ", " + data.WorkerID.VerbatimString(true) + ", " + _dafny.String(data.ClaimEpoch) + ", " + _dafny.String(data.LeaseUntil) + ", " + _dafny.String(data.Retries) + ")"
+		}
+	default:
+		{
+			return "<unexpected>"
+		}
+	}
+}
+
+func (_this EffectState) Equals(other EffectState) bool {
+	switch data1 := _this.Get_().(type) {
+	case EffectState_EffectState:
+		{
+			data2, ok := other.Get_().(EffectState_EffectState)
+			return ok && data1.EffectID.Equals(data2.EffectID) && data1.AttemptID.Equals(data2.AttemptID) && data1.Phase.Equals(data2.Phase) && data1.WorkerID.Equals(data2.WorkerID) && data1.ClaimEpoch.Cmp(data2.ClaimEpoch) == 0 && data1.LeaseUntil.Cmp(data2.LeaseUntil) == 0 && data1.Retries.Cmp(data2.Retries) == 0
+		}
+	default:
+		{
+			return false // unexpected
+		}
+	}
+}
+
+func (_this EffectState) EqualsGeneric(other interface{}) bool {
+	typed, ok := other.(EffectState)
+	return ok && _this.Equals(typed)
+}
+
+func Type_EffectState_() _dafny.TypeDescriptor {
+	return type_EffectState_{}
+}
+
+type type_EffectState_ struct {
+}
+
+func (_this type_EffectState_) Default() interface{} {
+	return Companion_EffectState_.Default()
+}
+
+func (_this type_EffectState_) String() string {
+	return "EffectReducer.EffectState"
+}
+func (_this EffectState) ParentTraits_() []*_dafny.TraitID {
+	return [](*_dafny.TraitID){}
+}
+
+var _ _dafny.TraitOffspring = EffectState{}
+
+// End of datatype EffectState
+
+// Definition of datatype Command
+type Command struct {
+	Data_Command_
+}
+
+func (_this Command) Get_() Data_Command_ {
+	return _this.Data_Command_
+}
+
+type Data_Command_ interface {
+	isCommand()
+}
+
+type CompanionStruct_Command_ struct {
+}
+
+var Companion_Command_ = CompanionStruct_Command_{}
+
+type Command_CommandClaimEffect struct {
+	EffectID        _dafny.Sequence
+	WorkerID        _dafny.Sequence
+	ExpectedVersion _dafny.Int
+	LeaseUntil      _dafny.Int
+	CurrentTime     _dafny.Int
+}
+
+func (Command_CommandClaimEffect) isCommand() {}
+
+func (CompanionStruct_Command_) Create_CommandClaimEffect_(EffectID _dafny.Sequence, WorkerID _dafny.Sequence, ExpectedVersion _dafny.Int, LeaseUntil _dafny.Int, CurrentTime _dafny.Int) Command {
+	return Command{Command_CommandClaimEffect{EffectID, WorkerID, ExpectedVersion, LeaseUntil, CurrentTime}}
+}
+
+func (_this Command) Is_CommandClaimEffect() bool {
+	_, ok := _this.Get_().(Command_CommandClaimEffect)
+	return ok
+}
+
+type Command_CommandObserveEffect struct {
+	EffectID   _dafny.Sequence
+	WorkerID   _dafny.Sequence
+	ClaimEpoch _dafny.Int
+	Outcome    Outcome
+}
+
+func (Command_CommandObserveEffect) isCommand() {}
+
+func (CompanionStruct_Command_) Create_CommandObserveEffect_(EffectID _dafny.Sequence, WorkerID _dafny.Sequence, ClaimEpoch _dafny.Int, Outcome Outcome) Command {
+	return Command{Command_CommandObserveEffect{EffectID, WorkerID, ClaimEpoch, Outcome}}
+}
+
+func (_this Command) Is_CommandObserveEffect() bool {
+	_, ok := _this.Get_().(Command_CommandObserveEffect)
+	return ok
+}
+
+type Command_CommandRetryEffect struct {
+	EffectID _dafny.Sequence
+}
+
+func (Command_CommandRetryEffect) isCommand() {}
+
+func (CompanionStruct_Command_) Create_CommandRetryEffect_(EffectID _dafny.Sequence) Command {
+	return Command{Command_CommandRetryEffect{EffectID}}
+}
+
+func (_this Command) Is_CommandRetryEffect() bool {
+	_, ok := _this.Get_().(Command_CommandRetryEffect)
+	return ok
+}
+
+type Command_CommandResolveUnknown struct {
+	EffectID _dafny.Sequence
+	Caps     CapabilityDescriptor
+}
+
+func (Command_CommandResolveUnknown) isCommand() {}
+
+func (CompanionStruct_Command_) Create_CommandResolveUnknown_(EffectID _dafny.Sequence, Caps CapabilityDescriptor) Command {
+	return Command{Command_CommandResolveUnknown{EffectID, Caps}}
+}
+
+func (_this Command) Is_CommandResolveUnknown() bool {
+	_, ok := _this.Get_().(Command_CommandResolveUnknown)
+	return ok
+}
+
+func (CompanionStruct_Command_) Default() Command {
+	return Companion_Command_.Create_CommandClaimEffect_(_dafny.EmptySeq, _dafny.EmptySeq, _dafny.Zero, _dafny.Zero, _dafny.Zero)
+}
+
+func (_this Command) Dtor_effectID() _dafny.Sequence {
+	switch data := _this.Get_().(type) {
+	case Command_CommandClaimEffect:
+		return data.EffectID
+	case Command_CommandObserveEffect:
+		return data.EffectID
+	case Command_CommandRetryEffect:
+		return data.EffectID
+	default:
+		return data.(Command_CommandResolveUnknown).EffectID
+	}
+}
+
+func (_this Command) Dtor_workerID() _dafny.Sequence {
+	switch data := _this.Get_().(type) {
+	case Command_CommandClaimEffect:
+		return data.WorkerID
+	default:
+		return data.(Command_CommandObserveEffect).WorkerID
+	}
+}
+
+func (_this Command) Dtor_expectedVersion() _dafny.Int {
+	return _this.Get_().(Command_CommandClaimEffect).ExpectedVersion
+}
+
+func (_this Command) Dtor_leaseUntil() _dafny.Int {
+	return _this.Get_().(Command_CommandClaimEffect).LeaseUntil
+}
+
+func (_this Command) Dtor_currentTime() _dafny.Int {
+	return _this.Get_().(Command_CommandClaimEffect).CurrentTime
+}
+
+func (_this Command) Dtor_claimEpoch() _dafny.Int {
+	return _this.Get_().(Command_CommandObserveEffect).ClaimEpoch
+}
+
+func (_this Command) Dtor_outcome() Outcome {
+	return _this.Get_().(Command_CommandObserveEffect).Outcome
+}
+
+func (_this Command) Dtor_caps() CapabilityDescriptor {
+	return _this.Get_().(Command_CommandResolveUnknown).Caps
+}
+
+func (_this Command) String() string {
+	switch data := _this.Get_().(type) {
+	case nil:
+		return "null"
+	case Command_CommandClaimEffect:
+		{
+			return "EffectReducer.Command.CommandClaimEffect" + "(" + data.EffectID.VerbatimString(true) + ", " + data.WorkerID.VerbatimString(true) + ", " + _dafny.String(data.ExpectedVersion) + ", " + _dafny.String(data.LeaseUntil) + ", " + _dafny.String(data.CurrentTime) + ")"
+		}
+	case Command_CommandObserveEffect:
+		{
+			return "EffectReducer.Command.CommandObserveEffect" + "(" + data.EffectID.VerbatimString(true) + ", " + data.WorkerID.VerbatimString(true) + ", " + _dafny.String(data.ClaimEpoch) + ", " + _dafny.String(data.Outcome) + ")"
+		}
+	case Command_CommandRetryEffect:
+		{
+			return "EffectReducer.Command.CommandRetryEffect" + "(" + data.EffectID.VerbatimString(true) + ")"
+		}
+	case Command_CommandResolveUnknown:
+		{
+			return "EffectReducer.Command.CommandResolveUnknown" + "(" + data.EffectID.VerbatimString(true) + ", " + _dafny.String(data.Caps) + ")"
+		}
+	default:
+		{
+			return "<unexpected>"
+		}
+	}
+}
+
+func (_this Command) Equals(other Command) bool {
+	switch data1 := _this.Get_().(type) {
+	case Command_CommandClaimEffect:
+		{
+			data2, ok := other.Get_().(Command_CommandClaimEffect)
+			return ok && data1.EffectID.Equals(data2.EffectID) && data1.WorkerID.Equals(data2.WorkerID) && data1.ExpectedVersion.Cmp(data2.ExpectedVersion) == 0 && data1.LeaseUntil.Cmp(data2.LeaseUntil) == 0 && data1.CurrentTime.Cmp(data2.CurrentTime) == 0
+		}
+	case Command_CommandObserveEffect:
+		{
+			data2, ok := other.Get_().(Command_CommandObserveEffect)
+			return ok && data1.EffectID.Equals(data2.EffectID) && data1.WorkerID.Equals(data2.WorkerID) && data1.ClaimEpoch.Cmp(data2.ClaimEpoch) == 0 && data1.Outcome.Equals(data2.Outcome)
+		}
+	case Command_CommandRetryEffect:
+		{
+			data2, ok := other.Get_().(Command_CommandRetryEffect)
+			return ok && data1.EffectID.Equals(data2.EffectID)
+		}
+	case Command_CommandResolveUnknown:
+		{
+			data2, ok := other.Get_().(Command_CommandResolveUnknown)
+			return ok && data1.EffectID.Equals(data2.EffectID) && data1.Caps.Equals(data2.Caps)
+		}
+	default:
+		{
+			return false // unexpected
+		}
+	}
+}
+
+func (_this Command) EqualsGeneric(other interface{}) bool {
+	typed, ok := other.(Command)
+	return ok && _this.Equals(typed)
+}
+
+func Type_Command_() _dafny.TypeDescriptor {
+	return type_Command_{}
+}
+
+type type_Command_ struct {
+}
+
+func (_this type_Command_) Default() interface{} {
+	return Companion_Command_.Default()
+}
+
+func (_this type_Command_) String() string {
+	return "EffectReducer.Command"
+}
+func (_this Command) ParentTraits_() []*_dafny.TraitID {
+	return [](*_dafny.TraitID){}
+}
+
+var _ _dafny.TraitOffspring = Command{}
+
+// End of datatype Command
+
+// Definition of datatype Event
+type Event struct {
+	Data_Event_
+}
+
+func (_this Event) Get_() Data_Event_ {
+	return _this.Data_Event_
+}
+
+type Data_Event_ interface {
+	isEvent()
+}
+
+type CompanionStruct_Event_ struct {
+}
+
+var Companion_Event_ = CompanionStruct_Event_{}
+
+type Event_EventEffectClaimed struct {
+	EffectID   _dafny.Sequence
+	WorkerID   _dafny.Sequence
+	ClaimEpoch _dafny.Int
+	LeaseUntil _dafny.Int
+}
+
+func (Event_EventEffectClaimed) isEvent() {}
+
+func (CompanionStruct_Event_) Create_EventEffectClaimed_(EffectID _dafny.Sequence, WorkerID _dafny.Sequence, ClaimEpoch _dafny.Int, LeaseUntil _dafny.Int) Event {
+	return Event{Event_EventEffectClaimed{EffectID, WorkerID, ClaimEpoch, LeaseUntil}}
+}
+
+func (_this Event) Is_EventEffectClaimed() bool {
+	_, ok := _this.Get_().(Event_EventEffectClaimed)
+	return ok
+}
+
+type Event_EventEffectObserved struct {
+	EffectID   _dafny.Sequence
+	ClaimEpoch _dafny.Int
+	Outcome    Outcome
+}
+
+func (Event_EventEffectObserved) isEvent() {}
+
+func (CompanionStruct_Event_) Create_EventEffectObserved_(EffectID _dafny.Sequence, ClaimEpoch _dafny.Int, Outcome Outcome) Event {
+	return Event{Event_EventEffectObserved{EffectID, ClaimEpoch, Outcome}}
+}
+
+func (_this Event) Is_EventEffectObserved() bool {
+	_, ok := _this.Get_().(Event_EventEffectObserved)
+	return ok
+}
+
+type Event_EventEffectRetried struct {
+	EffectID _dafny.Sequence
+}
+
+func (Event_EventEffectRetried) isEvent() {}
+
+func (CompanionStruct_Event_) Create_EventEffectRetried_(EffectID _dafny.Sequence) Event {
+	return Event{Event_EventEffectRetried{EffectID}}
+}
+
+func (_this Event) Is_EventEffectRetried() bool {
+	_, ok := _this.Get_().(Event_EventEffectRetried)
+	return ok
+}
+
+type Event_EventEffectTerminalized struct {
+	EffectID _dafny.Sequence
+	Reason   _dafny.Sequence
+}
+
+func (Event_EventEffectTerminalized) isEvent() {}
+
+func (CompanionStruct_Event_) Create_EventEffectTerminalized_(EffectID _dafny.Sequence, Reason _dafny.Sequence) Event {
+	return Event{Event_EventEffectTerminalized{EffectID, Reason}}
+}
+
+func (_this Event) Is_EventEffectTerminalized() bool {
+	_, ok := _this.Get_().(Event_EventEffectTerminalized)
+	return ok
+}
+
+type Event_EventEffectRejected struct {
+	EffectID _dafny.Sequence
+	Reason   _dafny.Sequence
+}
+
+func (Event_EventEffectRejected) isEvent() {}
+
+func (CompanionStruct_Event_) Create_EventEffectRejected_(EffectID _dafny.Sequence, Reason _dafny.Sequence) Event {
+	return Event{Event_EventEffectRejected{EffectID, Reason}}
+}
+
+func (_this Event) Is_EventEffectRejected() bool {
+	_, ok := _this.Get_().(Event_EventEffectRejected)
+	return ok
+}
+
+type Event_EventManualResolutionRequired struct {
+	EffectID _dafny.Sequence
+}
+
+func (Event_EventManualResolutionRequired) isEvent() {}
+
+func (CompanionStruct_Event_) Create_EventManualResolutionRequired_(EffectID _dafny.Sequence) Event {
+	return Event{Event_EventManualResolutionRequired{EffectID}}
+}
+
+func (_this Event) Is_EventManualResolutionRequired() bool {
+	_, ok := _this.Get_().(Event_EventManualResolutionRequired)
+	return ok
+}
+
+type Event_EventReconciliationRequired struct {
+	EffectID _dafny.Sequence
+}
+
+func (Event_EventReconciliationRequired) isEvent() {}
+
+func (CompanionStruct_Event_) Create_EventReconciliationRequired_(EffectID _dafny.Sequence) Event {
+	return Event{Event_EventReconciliationRequired{EffectID}}
+}
+
+func (_this Event) Is_EventReconciliationRequired() bool {
+	_, ok := _this.Get_().(Event_EventReconciliationRequired)
+	return ok
+}
+
+type Event_EventRetryAuthorized struct {
+	EffectID _dafny.Sequence
+}
+
+func (Event_EventRetryAuthorized) isEvent() {}
+
+func (CompanionStruct_Event_) Create_EventRetryAuthorized_(EffectID _dafny.Sequence) Event {
+	return Event{Event_EventRetryAuthorized{EffectID}}
+}
+
+func (_this Event) Is_EventRetryAuthorized() bool {
+	_, ok := _this.Get_().(Event_EventRetryAuthorized)
+	return ok
+}
+
+func (CompanionStruct_Event_) Default() Event {
+	return Companion_Event_.Create_EventEffectClaimed_(_dafny.EmptySeq, _dafny.EmptySeq, _dafny.Zero, _dafny.Zero)
+}
+
+func (_this Event) Dtor_effectID() _dafny.Sequence {
+	switch data := _this.Get_().(type) {
+	case Event_EventEffectClaimed:
+		return data.EffectID
+	case Event_EventEffectObserved:
+		return data.EffectID
+	case Event_EventEffectRetried:
+		return data.EffectID
+	case Event_EventEffectTerminalized:
+		return data.EffectID
+	case Event_EventEffectRejected:
+		return data.EffectID
+	case Event_EventManualResolutionRequired:
+		return data.EffectID
+	case Event_EventReconciliationRequired:
+		return data.EffectID
+	default:
+		return data.(Event_EventRetryAuthorized).EffectID
+	}
+}
+
+func (_this Event) Dtor_workerID() _dafny.Sequence {
+	return _this.Get_().(Event_EventEffectClaimed).WorkerID
+}
+
+func (_this Event) Dtor_claimEpoch() _dafny.Int {
+	switch data := _this.Get_().(type) {
+	case Event_EventEffectClaimed:
+		return data.ClaimEpoch
+	default:
+		return data.(Event_EventEffectObserved).ClaimEpoch
+	}
+}
+
+func (_this Event) Dtor_leaseUntil() _dafny.Int {
+	return _this.Get_().(Event_EventEffectClaimed).LeaseUntil
+}
+
+func (_this Event) Dtor_outcome() Outcome {
+	return _this.Get_().(Event_EventEffectObserved).Outcome
+}
+
+func (_this Event) Dtor_reason() _dafny.Sequence {
+	switch data := _this.Get_().(type) {
+	case Event_EventEffectTerminalized:
+		return data.Reason
+	default:
+		return data.(Event_EventEffectRejected).Reason
+	}
+}
+
+func (_this Event) String() string {
+	switch data := _this.Get_().(type) {
+	case nil:
+		return "null"
+	case Event_EventEffectClaimed:
+		{
+			return "EffectReducer.Event.EventEffectClaimed" + "(" + data.EffectID.VerbatimString(true) + ", " + data.WorkerID.VerbatimString(true) + ", " + _dafny.String(data.ClaimEpoch) + ", " + _dafny.String(data.LeaseUntil) + ")"
+		}
+	case Event_EventEffectObserved:
+		{
+			return "EffectReducer.Event.EventEffectObserved" + "(" + data.EffectID.VerbatimString(true) + ", " + _dafny.String(data.ClaimEpoch) + ", " + _dafny.String(data.Outcome) + ")"
+		}
+	case Event_EventEffectRetried:
+		{
+			return "EffectReducer.Event.EventEffectRetried" + "(" + data.EffectID.VerbatimString(true) + ")"
+		}
+	case Event_EventEffectTerminalized:
+		{
+			return "EffectReducer.Event.EventEffectTerminalized" + "(" + data.EffectID.VerbatimString(true) + ", " + data.Reason.VerbatimString(true) + ")"
+		}
+	case Event_EventEffectRejected:
+		{
+			return "EffectReducer.Event.EventEffectRejected" + "(" + data.EffectID.VerbatimString(true) + ", " + data.Reason.VerbatimString(true) + ")"
+		}
+	case Event_EventManualResolutionRequired:
+		{
+			return "EffectReducer.Event.EventManualResolutionRequired" + "(" + data.EffectID.VerbatimString(true) + ")"
+		}
+	case Event_EventReconciliationRequired:
+		{
+			return "EffectReducer.Event.EventReconciliationRequired" + "(" + data.EffectID.VerbatimString(true) + ")"
+		}
+	case Event_EventRetryAuthorized:
+		{
+			return "EffectReducer.Event.EventRetryAuthorized" + "(" + data.EffectID.VerbatimString(true) + ")"
+		}
+	default:
+		{
+			return "<unexpected>"
+		}
+	}
+}
+
+func (_this Event) Equals(other Event) bool {
+	switch data1 := _this.Get_().(type) {
+	case Event_EventEffectClaimed:
+		{
+			data2, ok := other.Get_().(Event_EventEffectClaimed)
+			return ok && data1.EffectID.Equals(data2.EffectID) && data1.WorkerID.Equals(data2.WorkerID) && data1.ClaimEpoch.Cmp(data2.ClaimEpoch) == 0 && data1.LeaseUntil.Cmp(data2.LeaseUntil) == 0
+		}
+	case Event_EventEffectObserved:
+		{
+			data2, ok := other.Get_().(Event_EventEffectObserved)
+			return ok && data1.EffectID.Equals(data2.EffectID) && data1.ClaimEpoch.Cmp(data2.ClaimEpoch) == 0 && data1.Outcome.Equals(data2.Outcome)
+		}
+	case Event_EventEffectRetried:
+		{
+			data2, ok := other.Get_().(Event_EventEffectRetried)
+			return ok && data1.EffectID.Equals(data2.EffectID)
+		}
+	case Event_EventEffectTerminalized:
+		{
+			data2, ok := other.Get_().(Event_EventEffectTerminalized)
+			return ok && data1.EffectID.Equals(data2.EffectID) && data1.Reason.Equals(data2.Reason)
+		}
+	case Event_EventEffectRejected:
+		{
+			data2, ok := other.Get_().(Event_EventEffectRejected)
+			return ok && data1.EffectID.Equals(data2.EffectID) && data1.Reason.Equals(data2.Reason)
+		}
+	case Event_EventManualResolutionRequired:
+		{
+			data2, ok := other.Get_().(Event_EventManualResolutionRequired)
+			return ok && data1.EffectID.Equals(data2.EffectID)
+		}
+	case Event_EventReconciliationRequired:
+		{
+			data2, ok := other.Get_().(Event_EventReconciliationRequired)
+			return ok && data1.EffectID.Equals(data2.EffectID)
+		}
+	case Event_EventRetryAuthorized:
+		{
+			data2, ok := other.Get_().(Event_EventRetryAuthorized)
+			return ok && data1.EffectID.Equals(data2.EffectID)
+		}
+	default:
+		{
+			return false // unexpected
+		}
+	}
+}
+
+func (_this Event) EqualsGeneric(other interface{}) bool {
+	typed, ok := other.(Event)
+	return ok && _this.Equals(typed)
+}
+
+func Type_Event_() _dafny.TypeDescriptor {
+	return type_Event_{}
+}
+
+type type_Event_ struct {
+}
+
+func (_this type_Event_) Default() interface{} {
+	return Companion_Event_.Default()
+}
+
+func (_this type_Event_) String() string {
+	return "EffectReducer.Event"
+}
+func (_this Event) ParentTraits_() []*_dafny.TraitID {
+	return [](*_dafny.TraitID){}
+}
+
+var _ _dafny.TraitOffspring = Event{}
+
+// End of datatype Event
+
+// Definition of datatype DecisionStatus
+type DecisionStatus struct {
+	Data_DecisionStatus_
+}
+
+func (_this DecisionStatus) Get_() Data_DecisionStatus_ {
+	return _this.Data_DecisionStatus_
+}
+
+type Data_DecisionStatus_ interface {
+	isDecisionStatus()
+}
+
+type CompanionStruct_DecisionStatus_ struct {
+}
+
+var Companion_DecisionStatus_ = CompanionStruct_DecisionStatus_{}
+
+type DecisionStatus_Accepted struct {
+}
+
+func (DecisionStatus_Accepted) isDecisionStatus() {}
+
+func (CompanionStruct_DecisionStatus_) Create_Accepted_() DecisionStatus {
+	return DecisionStatus{DecisionStatus_Accepted{}}
+}
+
+func (_this DecisionStatus) Is_Accepted() bool {
+	_, ok := _this.Get_().(DecisionStatus_Accepted)
+	return ok
+}
+
+type DecisionStatus_Rejected struct {
+}
+
+func (DecisionStatus_Rejected) isDecisionStatus() {}
+
+func (CompanionStruct_DecisionStatus_) Create_Rejected_() DecisionStatus {
+	return DecisionStatus{DecisionStatus_Rejected{}}
+}
+
+func (_this DecisionStatus) Is_Rejected() bool {
+	_, ok := _this.Get_().(DecisionStatus_Rejected)
+	return ok
+}
+
+type DecisionStatus_NoOp struct {
+}
+
+func (DecisionStatus_NoOp) isDecisionStatus() {}
+
+func (CompanionStruct_DecisionStatus_) Create_NoOp_() DecisionStatus {
+	return DecisionStatus{DecisionStatus_NoOp{}}
+}
+
+func (_this DecisionStatus) Is_NoOp() bool {
+	_, ok := _this.Get_().(DecisionStatus_NoOp)
+	return ok
+}
+
+func (CompanionStruct_DecisionStatus_) Default() DecisionStatus {
+	return Companion_DecisionStatus_.Create_Accepted_()
+}
+
+func (_ CompanionStruct_DecisionStatus_) AllSingletonConstructors() _dafny.Iterator {
+	i := -1
+	return func() (interface{}, bool) {
+		i++
+		switch i {
+		case 0:
+			return Companion_DecisionStatus_.Create_Accepted_(), true
+		case 1:
+			return Companion_DecisionStatus_.Create_Rejected_(), true
+		case 2:
+			return Companion_DecisionStatus_.Create_NoOp_(), true
+		default:
+			return DecisionStatus{}, false
+		}
+	}
+}
+
+func (_this DecisionStatus) String() string {
+	switch _this.Get_().(type) {
+	case nil:
+		return "null"
+	case DecisionStatus_Accepted:
+		{
+			return "EffectReducer.DecisionStatus.Accepted"
+		}
+	case DecisionStatus_Rejected:
+		{
+			return "EffectReducer.DecisionStatus.Rejected"
+		}
+	case DecisionStatus_NoOp:
+		{
+			return "EffectReducer.DecisionStatus.NoOp"
+		}
+	default:
+		{
+			return "<unexpected>"
+		}
+	}
+}
+
+func (_this DecisionStatus) Equals(other DecisionStatus) bool {
+	switch _this.Get_().(type) {
+	case DecisionStatus_Accepted:
+		{
+			_, ok := other.Get_().(DecisionStatus_Accepted)
+			return ok
+		}
+	case DecisionStatus_Rejected:
+		{
+			_, ok := other.Get_().(DecisionStatus_Rejected)
+			return ok
+		}
+	case DecisionStatus_NoOp:
+		{
+			_, ok := other.Get_().(DecisionStatus_NoOp)
+			return ok
+		}
+	default:
+		{
+			return false // unexpected
+		}
+	}
+}
+
+func (_this DecisionStatus) EqualsGeneric(other interface{}) bool {
+	typed, ok := other.(DecisionStatus)
+	return ok && _this.Equals(typed)
+}
+
+func Type_DecisionStatus_() _dafny.TypeDescriptor {
+	return type_DecisionStatus_{}
+}
+
+type type_DecisionStatus_ struct {
+}
+
+func (_this type_DecisionStatus_) Default() interface{} {
+	return Companion_DecisionStatus_.Default()
+}
+
+func (_this type_DecisionStatus_) String() string {
+	return "EffectReducer.DecisionStatus"
+}
+func (_this DecisionStatus) ParentTraits_() []*_dafny.TraitID {
+	return [](*_dafny.TraitID){}
+}
+
+var _ _dafny.TraitOffspring = DecisionStatus{}
+
+// End of datatype DecisionStatus
+
+// Definition of datatype Decision
+type Decision struct {
+	Data_Decision_
+}
+
+func (_this Decision) Get_() Data_Decision_ {
+	return _this.Data_Decision_
+}
+
+type Data_Decision_ interface {
+	isDecision()
+}
+
+type CompanionStruct_Decision_ struct {
+}
+
+var Companion_Decision_ = CompanionStruct_Decision_{}
+
+type Decision_Decision struct {
+	Status DecisionStatus
+	Events _dafny.Sequence
+}
+
+func (Decision_Decision) isDecision() {}
+
+func (CompanionStruct_Decision_) Create_Decision_(Status DecisionStatus, Events _dafny.Sequence) Decision {
+	return Decision{Decision_Decision{Status, Events}}
+}
+
+func (_this Decision) Is_Decision() bool {
+	_, ok := _this.Get_().(Decision_Decision)
+	return ok
+}
+
+func (CompanionStruct_Decision_) Default() Decision {
+	return Companion_Decision_.Create_Decision_(Companion_DecisionStatus_.Default(), _dafny.EmptySeq)
+}
+
+func (_this Decision) Dtor_status() DecisionStatus {
+	return _this.Get_().(Decision_Decision).Status
+}
+
+func (_this Decision) Dtor_events() _dafny.Sequence {
+	return _this.Get_().(Decision_Decision).Events
+}
+
+func (_this Decision) String() string {
+	switch data := _this.Get_().(type) {
+	case nil:
+		return "null"
+	case Decision_Decision:
+		{
+			return "EffectReducer.Decision.Decision" + "(" + _dafny.String(data.Status) + ", " + _dafny.String(data.Events) + ")"
+		}
+	default:
+		{
+			return "<unexpected>"
+		}
+	}
+}
+
+func (_this Decision) Equals(other Decision) bool {
+	switch data1 := _this.Get_().(type) {
+	case Decision_Decision:
+		{
+			data2, ok := other.Get_().(Decision_Decision)
+			return ok && data1.Status.Equals(data2.Status) && data1.Events.Equals(data2.Events)
+		}
+	default:
+		{
+			return false // unexpected
+		}
+	}
+}
+
+func (_this Decision) EqualsGeneric(other interface{}) bool {
+	typed, ok := other.(Decision)
+	return ok && _this.Equals(typed)
+}
+
+func Type_Decision_() _dafny.TypeDescriptor {
+	return type_Decision_{}
+}
+
+type type_Decision_ struct {
+}
+
+func (_this type_Decision_) Default() interface{} {
+	return Companion_Decision_.Default()
+}
+
+func (_this type_Decision_) String() string {
+	return "EffectReducer.Decision"
+}
+func (_this Decision) ParentTraits_() []*_dafny.TraitID {
+	return [](*_dafny.TraitID){}
+}
+
+var _ _dafny.TraitOffspring = Decision{}
+
+// End of datatype Decision
