internal/dafny_reducer/Reducer.go
@@ -1,155 +1,157 @@
 // Package Reducer
 // Dafny module Reducer compiled into Go
 
-package Reducer
+package dafny_reducer
 
 import (
-  os "os"
-  _dafny "github.com/dafny-lang/DafnyRuntimeGo/v4/dafny"
-  m__System "github.com/dafny-lang/DafnyRuntimeGo/v4/System_"
+	m__System "github.com/dafny-lang/DafnyRuntimeGo/v4/System_"
+	_dafny "github.com/dafny-lang/DafnyRuntimeGo/v4/dafny"
+	os "os"
 )
+
 var _ = os.Args
 var _ _dafny.Dummy__
 var _ m__System.Dummy__
 
 type Dummy__ struct{}
 
-
 // Definition of class Default__
 type Default__ struct {
-  dummy byte
+	dummy byte
 }
 
 func New_Default___() *Default__ {
-  _this := Default__{}
+	_this := Default__{}
 
-  return &_this
+	return &_this
 }
 
 type CompanionStruct_Default___ struct {
 }
-var Companion_Default___ = CompanionStruct_Default___ {
-}
+
+var Companion_Default___ = CompanionStruct_Default___{}
 
 func (_this *Default__) Equals(other *Default__) bool {
-  return _this == other
+	return _this == other
 }
 
 func (_this *Default__) EqualsGeneric(x interface{}) bool {
-  other, ok := x.(*Default__)
-  return ok && _this.Equals(other)
+	other, ok := x.(*Default__)
+	return ok && _this.Equals(other)
 }
 
 func (*Default__) String() string {
-  return "_module.Default__"
+	return "_module.Default__"
 }
 func (_this *Default__) ParentTraits_() []*_dafny.TraitID {
-  return [](*_dafny.TraitID){};
+	return [](*_dafny.TraitID){}
 }
+
 var _ _dafny.TraitOffspring = &Default__{}
 
 func (_static *CompanionStruct_Default___) Decide(state AttemptState, cmd Command) Decision {
-  var _source0 Command = cmd
-  _ = _source0
-  {
-    if (_source0.Is_CommandConclude()) {
-      var _0_attemptID _dafny.Sequence = _source0.Get_().(Command_CommandConclude).AttemptID
-      _ = _0_attemptID
-      if (((state).Dtor_phase()).Equals(Companion_Phase_.Create_Concluded_())) {
-        return Companion_Decision_.Create_Decision_(Companion_DecisionStatus_.Create_NoOp_(), _dafny.SeqOf(), _dafny.SeqOf())
-      } else {
-        return Companion_Decision_.Create_Decision_(Companion_DecisionStatus_.Create_Accepted_(), _dafny.SeqOf(Companion_Event_.Create_EventConcluded_(_0_attemptID)), _dafny.SeqOf())
-      }
-    }
-  }
-  {
-    if (_source0.Is_CommandUnknown()) {
-      var _1_attemptID _dafny.Sequence = _source0.Get_().(Command_CommandUnknown).AttemptID
-      _ = _1_attemptID
-      return Companion_Decision_.Create_Decision_(Companion_DecisionStatus_.Create_Rejected_(), _dafny.SeqOf(), _dafny.SeqOf())
-    }
-  }
-  {
-    var _2_attemptID _dafny.Sequence = _source0.Get_().(Command_CommandProposeRecovery).AttemptID
-    _ = _2_attemptID
-    var _3_idempotencyKey _dafny.Sequence = _source0.Get_().(Command_CommandProposeRecovery).IdempotencyKey
-    _ = _3_idempotencyKey
-    var _4_version _dafny.Int = _source0.Get_().(Command_CommandProposeRecovery).Version
-    _ = _4_version
-    if (((_4_version).Sign() == 1) && ((_4_version).Cmp((state).Dtor_version()) < 0)) {
-      return Companion_Decision_.Create_Decision_(Companion_DecisionStatus_.Create_Rejected_(), _dafny.SeqOf(Companion_Event_.Create_EventRecoveryRejected_(_2_attemptID, _dafny.UnicodeSeqOfUtf8Bytes("stale command"))), _dafny.SeqOf())
-    } else if (((state).Dtor_phase()).Equals(Companion_Phase_.Create_Concluded_())) {
-      return Companion_Decision_.Create_Decision_(Companion_DecisionStatus_.Create_Rejected_(), _dafny.SeqOf(Companion_Event_.Create_EventRecoveryRejected_(_2_attemptID, _dafny.UnicodeSeqOfUtf8Bytes("attempt already concluded"))), _dafny.SeqOf())
-    } else if (((state).Dtor_processedCmdKeys()).Contains(_3_idempotencyKey)) {
-      return Companion_Decision_.Create_Decision_(Companion_DecisionStatus_.Create_NoOp_(), _dafny.SeqOf(), _dafny.SeqOf())
-    } else if (((state).Dtor_recoveryDispatches()).Cmp(_dafny.IntOfInt64(2)) >= 0) {
-      return Companion_Decision_.Create_Decision_(Companion_DecisionStatus_.Create_Rejected_(), _dafny.SeqOf(Companion_Event_.Create_EventRecoveryRejected_(_2_attemptID, _dafny.UnicodeSeqOfUtf8Bytes("recovery limit reached"))), _dafny.SeqOf())
-    } else {
-      var _5_effectID _dafny.Sequence = _dafny.Companion_Sequence_.Concatenate(_dafny.Companion_Sequence_.Concatenate(_2_attemptID, _dafny.UnicodeSeqOfUtf8Bytes("-effect-")), _3_idempotencyKey)
-      _ = _5_effectID
-      if (((state).Dtor_dispatchedEffects()).Contains(_5_effectID)) {
-        return Companion_Decision_.Create_Decision_(Companion_DecisionStatus_.Create_Rejected_(), _dafny.SeqOf(Companion_Event_.Create_EventRecoveryRejected_(_2_attemptID, _dafny.UnicodeSeqOfUtf8Bytes("effect collision"))), _dafny.SeqOf())
-      } else {
-        return Companion_Decision_.Create_Decision_(Companion_DecisionStatus_.Create_Accepted_(), _dafny.SeqOf(Companion_Event_.Create_EventRecoveryDispatched_(_2_attemptID, _5_effectID, ((state).Dtor_recoveryDispatches()).Plus(_dafny.One), _3_idempotencyKey)), _dafny.SeqOf(Companion_EffectIntent_.Create_EffectIntent_(_2_attemptID, _5_effectID, ((state).Dtor_recoveryDispatches()).Plus(_dafny.One))))
-      }
-    }
-  }
+	var _source0 Command = cmd
+	_ = _source0
+	{
+		if _source0.Is_CommandConclude() {
+			var _0_attemptID _dafny.Sequence = _source0.Get_().(Command_CommandConclude).AttemptID
+			_ = _0_attemptID
+			if ((state).Dtor_phase()).Equals(Companion_Phase_.Create_Concluded_()) {
+				return Companion_Decision_.Create_Decision_(Companion_DecisionStatus_.Create_NoOp_(), _dafny.SeqOf(), _dafny.SeqOf())
+			} else {
+				return Companion_Decision_.Create_Decision_(Companion_DecisionStatus_.Create_Accepted_(), _dafny.SeqOf(Companion_Event_.Create_EventConcluded_(_0_attemptID)), _dafny.SeqOf())
+			}
+		}
+	}
+	{
+		if _source0.Is_CommandUnknown() {
+			var _1_attemptID _dafny.Sequence = _source0.Get_().(Command_CommandUnknown).AttemptID
+			_ = _1_attemptID
+			return Companion_Decision_.Create_Decision_(Companion_DecisionStatus_.Create_Rejected_(), _dafny.SeqOf(), _dafny.SeqOf())
+		}
+	}
+	{
+		var _2_attemptID _dafny.Sequence = _source0.Get_().(Command_CommandProposeRecovery).AttemptID
+		_ = _2_attemptID
+		var _3_idempotencyKey _dafny.Sequence = _source0.Get_().(Command_CommandProposeRecovery).IdempotencyKey
+		_ = _3_idempotencyKey
+		var _4_version _dafny.Int = _source0.Get_().(Command_CommandProposeRecovery).Version
+		_ = _4_version
+		if ((_4_version).Sign() == 1) && ((_4_version).Cmp((state).Dtor_version()) < 0) {
+			return Companion_Decision_.Create_Decision_(Companion_DecisionStatus_.Create_Rejected_(), _dafny.SeqOf(Companion_Event_.Create_EventRecoveryRejected_(_2_attemptID, _dafny.UnicodeSeqOfUtf8Bytes("stale command"))), _dafny.SeqOf())
+		} else if ((state).Dtor_phase()).Equals(Companion_Phase_.Create_Concluded_()) {
+			return Companion_Decision_.Create_Decision_(Companion_DecisionStatus_.Create_Rejected_(), _dafny.SeqOf(Companion_Event_.Create_EventRecoveryRejected_(_2_attemptID, _dafny.UnicodeSeqOfUtf8Bytes("attempt already concluded"))), _dafny.SeqOf())
+		} else if ((state).Dtor_processedCmdKeys()).Contains(_3_idempotencyKey) {
+			return Companion_Decision_.Create_Decision_(Companion_DecisionStatus_.Create_NoOp_(), _dafny.SeqOf(), _dafny.SeqOf())
+		} else if ((state).Dtor_recoveryDispatches()).Cmp(_dafny.IntOfInt64(2)) >= 0 {
+			return Companion_Decision_.Create_Decision_(Companion_DecisionStatus_.Create_Rejected_(), _dafny.SeqOf(Companion_Event_.Create_EventRecoveryRejected_(_2_attemptID, _dafny.UnicodeSeqOfUtf8Bytes("recovery limit reached"))), _dafny.SeqOf())
+		} else {
+			var _5_effectID _dafny.Sequence = _dafny.Companion_Sequence_.Concatenate(_dafny.Companion_Sequence_.Concatenate(_2_attemptID, _dafny.UnicodeSeqOfUtf8Bytes("-effect-")), _3_idempotencyKey)
+			_ = _5_effectID
+			if ((state).Dtor_dispatchedEffects()).Contains(_5_effectID) {
+				return Companion_Decision_.Create_Decision_(Companion_DecisionStatus_.Create_Rejected_(), _dafny.SeqOf(Companion_Event_.Create_EventRecoveryRejected_(_2_attemptID, _dafny.UnicodeSeqOfUtf8Bytes("effect collision"))), _dafny.SeqOf())
+			} else {
+				return Companion_Decision_.Create_Decision_(Companion_DecisionStatus_.Create_Accepted_(), _dafny.SeqOf(Companion_Event_.Create_EventRecoveryDispatched_(_2_attemptID, _5_effectID, ((state).Dtor_recoveryDispatches()).Plus(_dafny.One), _3_idempotencyKey)), _dafny.SeqOf(Companion_EffectIntent_.Create_EffectIntent_(_2_attemptID, _5_effectID, ((state).Dtor_recoveryDispatches()).Plus(_dafny.One))))
+			}
+		}
+	}
 }
 func (_static *CompanionStruct_Default___) Apply(state AttemptState, event Event) AttemptState {
-  var _source0 Event = event
-  _ = _source0
-  {
-    if (_source0.Is_EventConcluded()) {
-      return Companion_AttemptState_.Create_AttemptState_(Companion_Phase_.Create_Concluded_(), (state).Dtor_recoveryDispatches(), (state).Dtor_dispatchedEffects(), (state).Dtor_processedCmdKeys(), (state).Dtor_version())
-    }
-  }
-  {
-    if (_source0.Is_EventRecoveryDispatched()) {
-      var _0_effectID _dafny.Sequence = _source0.Get_().(Event_EventRecoveryDispatched).EffectID
-      _ = _0_effectID
-      var _1_idempotencyKey _dafny.Sequence = _source0.Get_().(Event_EventRecoveryDispatched).IdempotencyKey
-      _ = _1_idempotencyKey
-      return Companion_AttemptState_.Create_AttemptState_(Companion_Phase_.Create_Recovering_(), ((state).Dtor_recoveryDispatches()).Plus(_dafny.One), ((state).Dtor_dispatchedEffects()).Union(_dafny.SetOf(_0_effectID)), ((state).Dtor_processedCmdKeys()).Union(_dafny.SetOf(_1_idempotencyKey)), (state).Dtor_version())
-    }
-  }
-  {
-    return state
-  }
+	var _source0 Event = event
+	_ = _source0
+	{
+		if _source0.Is_EventConcluded() {
+			return Companion_AttemptState_.Create_AttemptState_(Companion_Phase_.Create_Concluded_(), (state).Dtor_recoveryDispatches(), (state).Dtor_dispatchedEffects(), (state).Dtor_processedCmdKeys(), (state).Dtor_version())
+		}
+	}
+	{
+		if _source0.Is_EventRecoveryDispatched() {
+			var _0_effectID _dafny.Sequence = _source0.Get_().(Event_EventRecoveryDispatched).EffectID
+			_ = _0_effectID
+			var _1_idempotencyKey _dafny.Sequence = _source0.Get_().(Event_EventRecoveryDispatched).IdempotencyKey
+			_ = _1_idempotencyKey
+			return Companion_AttemptState_.Create_AttemptState_(Companion_Phase_.Create_Recovering_(), ((state).Dtor_recoveryDispatches()).Plus(_dafny.One), ((state).Dtor_dispatchedEffects()).Union(_dafny.SetOf(_0_effectID)), ((state).Dtor_processedCmdKeys()).Union(_dafny.SetOf(_1_idempotencyKey)), (state).Dtor_version())
+		}
+	}
+	{
+		return state
+	}
 }
 func (_static *CompanionStruct_Default___) ApplyBatch(state AttemptState, events _dafny.Sequence) AttemptState {
-  goto TAIL_CALL_START
-  TAIL_CALL_START:
-  if ((_dafny.IntOfUint32((events).Cardinality())).Sign() == 0) {
-    return state
-  } else {
-    var _in0 AttemptState = Companion_Default___.Apply(state, (events).Select(0).(Event))
-    _ = _in0
-    var _in1 _dafny.Sequence = (events).Drop(1)
-    _ = _in1
-    state = _in0
-    events = _in1
-    goto TAIL_CALL_START
-  }
+	goto TAIL_CALL_START
+TAIL_CALL_START:
+	if (_dafny.IntOfUint32((events).Cardinality())).Sign() == 0 {
+		return state
+	} else {
+		var _in0 AttemptState = Companion_Default___.Apply(state, (events).Select(0).(Event))
+		_ = _in0
+		var _in1 _dafny.Sequence = (events).Drop(1)
+		_ = _in1
+		state = _in0
+		events = _in1
+		goto TAIL_CALL_START
+	}
 }
+
 // End of class Default__
 
 // Definition of datatype Phase
 type Phase struct {
-  Data_Phase_
+	Data_Phase_
 }
 
 func (_this Phase) Get_() Data_Phase_ {
-  return _this.Data_Phase_
+	return _this.Data_Phase_
 }
 
 type Data_Phase_ interface {
-  isPhase()
+	isPhase()
 }
 
 type CompanionStruct_Phase_ struct {
 }
-var Companion_Phase_ = CompanionStruct_Phase_ {
-}
+
+var Companion_Phase_ = CompanionStruct_Phase_{}
 
 type Phase_Active struct {
 }
@@ -157,12 +159,12 @@ type Phase_Active struct {
 func (Phase_Active) isPhase() {}
 
 func (CompanionStruct_Phase_) Create_Active_() Phase {
-  return Phase{Phase_Active{}}
+	return Phase{Phase_Active{}}
 }
 
 func (_this Phase) Is_Active() bool {
-  _, ok := _this.Get_().(Phase_Active)
-  return ok
+	_, ok := _this.Get_().(Phase_Active)
+	return ok
 }
 
 type Phase_Recovering struct {
@@ -171,12 +173,12 @@ type Phase_Recovering struct {
 func (Phase_Recovering) isPhase() {}
 
 func (CompanionStruct_Phase_) Create_Recovering_() Phase {
-  return Phase{Phase_Recovering{}}
+	return Phase{Phase_Recovering{}}
 }
 
 func (_this Phase) Is_Recovering() bool {
-  _, ok := _this.Get_().(Phase_Recovering)
-  return ok
+	_, ok := _this.Get_().(Phase_Recovering)
+	return ok
 }
 
 type Phase_Concluded struct {
@@ -185,632 +187,684 @@ type Phase_Concluded struct {
 func (Phase_Concluded) isPhase() {}
 
 func (CompanionStruct_Phase_) Create_Concluded_() Phase {
-  return Phase{Phase_Concluded{}}
+	return Phase{Phase_Concluded{}}
 }
 
 func (_this Phase) Is_Concluded() bool {
-  _, ok := _this.Get_().(Phase_Concluded)
-  return ok
+	_, ok := _this.Get_().(Phase_Concluded)
+	return ok
 }
 
 func (CompanionStruct_Phase_) Default() Phase {
-  return Companion_Phase_.Create_Active_()
+	return Companion_Phase_.Create_Active_()
 }
 
 func (_ CompanionStruct_Phase_) AllSingletonConstructors() _dafny.Iterator {
-  i := -1
-  return func() (interface{}, bool) {
-    i++
-    switch i {
-      case 0: return Companion_Phase_.Create_Active_(), true
-      case 1: return Companion_Phase_.Create_Recovering_(), true
-      case 2: return Companion_Phase_.Create_Concluded_(), true
-      default: return Phase{}, false
-    }
-  }
+	i := -1
+	return func() (interface{}, bool) {
+		i++
+		switch i {
+		case 0:
+			return Companion_Phase_.Create_Active_(), true
+		case 1:
+			return Companion_Phase_.Create_Recovering_(), true
+		case 2:
+			return Companion_Phase_.Create_Concluded_(), true
+		default:
+			return Phase{}, false
+		}
+	}
 }
 
 func (_this Phase) String() string {
-  switch _this.Get_().(type) {
-    case nil: return "null"
-    case Phase_Active: {
-      return "Reducer.Phase.Active"
-    }
-    case Phase_Recovering: {
-      return "Reducer.Phase.Recovering"
-    }
-    case Phase_Concluded: {
-      return "Reducer.Phase.Concluded"
-    }
-    default: {
-      return "<unexpected>"
-    }
-  }
+	switch _this.Get_().(type) {
+	case nil:
+		return "null"
+	case Phase_Active:
+		{
+			return "Reducer.Phase.Active"
+		}
+	case Phase_Recovering:
+		{
+			return "Reducer.Phase.Recovering"
+		}
+	case Phase_Concluded:
+		{
+			return "Reducer.Phase.Concluded"
+		}
+	default:
+		{
+			return "<unexpected>"
+		}
+	}
 }
 
 func (_this Phase) Equals(other Phase) bool {
-  switch _this.Get_().(type) {
-    case Phase_Active: {
-      _, ok := other.Get_().(Phase_Active)
-      return ok
-    }
-    case Phase_Recovering: {
-      _, ok := other.Get_().(Phase_Recovering)
-      return ok
-    }
-    case Phase_Concluded: {
-      _, ok := other.Get_().(Phase_Concluded)
-      return ok
-    }
-    default: {
-      return false; // unexpected
-    }
-  }
+	switch _this.Get_().(type) {
+	case Phase_Active:
+		{
+			_, ok := other.Get_().(Phase_Active)
+			return ok
+		}
+	case Phase_Recovering:
+		{
+			_, ok := other.Get_().(Phase_Recovering)
+			return ok
+		}
+	case Phase_Concluded:
+		{
+			_, ok := other.Get_().(Phase_Concluded)
+			return ok
+		}
+	default:
+		{
+			return false // unexpected
+		}
+	}
 }
 
 func (_this Phase) EqualsGeneric(other interface{}) bool {
-  typed, ok := other.(Phase)
-  return ok && _this.Equals(typed)
+	typed, ok := other.(Phase)
+	return ok && _this.Equals(typed)
 }
 
 func Type_Phase_() _dafny.TypeDescriptor {
-  return type_Phase_{}
+	return type_Phase_{}
 }
 
 type type_Phase_ struct {
 }
 
 func (_this type_Phase_) Default() interface{} {
-  return Companion_Phase_.Default();
+	return Companion_Phase_.Default()
 }
 
 func (_this type_Phase_) String() string {
-  return "Reducer.Phase"
+	return "Reducer.Phase"
 }
 func (_this Phase) ParentTraits_() []*_dafny.TraitID {
-  return [](*_dafny.TraitID){};
+	return [](*_dafny.TraitID){}
 }
+
 var _ _dafny.TraitOffspring = Phase{}
 
 // End of datatype Phase
 
 // Definition of datatype AttemptState
 type AttemptState struct {
-  Data_AttemptState_
+	Data_AttemptState_
 }
 
 func (_this AttemptState) Get_() Data_AttemptState_ {
-  return _this.Data_AttemptState_
+	return _this.Data_AttemptState_
 }
 
 type Data_AttemptState_ interface {
-  isAttemptState()
+	isAttemptState()
 }
 
 type CompanionStruct_AttemptState_ struct {
 }
-var Companion_AttemptState_ = CompanionStruct_AttemptState_ {
-}
+
+var Companion_AttemptState_ = CompanionStruct_AttemptState_{}
 
 type AttemptState_AttemptState struct {
-  Phase Phase
-  RecoveryDispatches _dafny.Int
-  DispatchedEffects _dafny.Set
-  ProcessedCmdKeys _dafny.Set
-  Version _dafny.Int
+	Phase              Phase
+	RecoveryDispatches _dafny.Int
+	DispatchedEffects  _dafny.Set
+	ProcessedCmdKeys   _dafny.Set
+	Version            _dafny.Int
 }
 
 func (AttemptState_AttemptState) isAttemptState() {}
 
 func (CompanionStruct_AttemptState_) Create_AttemptState_(Phase Phase, RecoveryDispatches _dafny.Int, DispatchedEffects _dafny.Set, ProcessedCmdKeys _dafny.Set, Version _dafny.Int) AttemptState {
-  return AttemptState{AttemptState_AttemptState{Phase, RecoveryDispatches, DispatchedEffects, ProcessedCmdKeys, Version}}
+	return AttemptState{AttemptState_AttemptState{Phase, RecoveryDispatches, DispatchedEffects, ProcessedCmdKeys, Version}}
 }
 
 func (_this AttemptState) Is_AttemptState() bool {
-  _, ok := _this.Get_().(AttemptState_AttemptState)
-  return ok
+	_, ok := _this.Get_().(AttemptState_AttemptState)
+	return ok
 }
 
 func (CompanionStruct_AttemptState_) Default() AttemptState {
-  return Companion_AttemptState_.Create_AttemptState_(Companion_Phase_.Default(), _dafny.Zero, _dafny.EmptySet, _dafny.EmptySet, _dafny.Zero)
+	return Companion_AttemptState_.Create_AttemptState_(Companion_Phase_.Default(), _dafny.Zero, _dafny.EmptySet, _dafny.EmptySet, _dafny.Zero)
 }
 
 func (_this AttemptState) Dtor_phase() Phase {
-  return _this.Get_().(AttemptState_AttemptState).Phase
+	return _this.Get_().(AttemptState_AttemptState).Phase
 }
 
 func (_this AttemptState) Dtor_recoveryDispatches() _dafny.Int {
-  return _this.Get_().(AttemptState_AttemptState).RecoveryDispatches
+	return _this.Get_().(AttemptState_AttemptState).RecoveryDispatches
 }
 
 func (_this AttemptState) Dtor_dispatchedEffects() _dafny.Set {
-  return _this.Get_().(AttemptState_AttemptState).DispatchedEffects
+	return _this.Get_().(AttemptState_AttemptState).DispatchedEffects
 }
 
 func (_this AttemptState) Dtor_processedCmdKeys() _dafny.Set {
-  return _this.Get_().(AttemptState_AttemptState).ProcessedCmdKeys
+	return _this.Get_().(AttemptState_AttemptState).ProcessedCmdKeys
 }
 
 func (_this AttemptState) Dtor_version() _dafny.Int {
-  return _this.Get_().(AttemptState_AttemptState).Version
+	return _this.Get_().(AttemptState_AttemptState).Version
 }
 
 func (_this AttemptState) String() string {
-  switch data := _this.Get_().(type) {
-    case nil: return "null"
-    case AttemptState_AttemptState: {
-      return "Reducer.AttemptState.AttemptState" + "(" + _dafny.String(data.Phase) + ", " + _dafny.String(data.RecoveryDispatches) + ", " + _dafny.String(data.DispatchedEffects) + ", " + _dafny.String(data.ProcessedCmdKeys) + ", " + _dafny.String(data.Version) + ")"
-    }
-    default: {
-      return "<unexpected>"
-    }
-  }
+	switch data := _this.Get_().(type) {
+	case nil:
+		return "null"
+	case AttemptState_AttemptState:
+		{
+			return "Reducer.AttemptState.AttemptState" + "(" + _dafny.String(data.Phase) + ", " + _dafny.String(data.RecoveryDispatches) + ", " + _dafny.String(data.DispatchedEffects) + ", " + _dafny.String(data.ProcessedCmdKeys) + ", " + _dafny.String(data.Version) + ")"
+		}
+	default:
+		{
+			return "<unexpected>"
+		}
+	}
 }
 
 func (_this AttemptState) Equals(other AttemptState) bool {
-  switch data1 := _this.Get_().(type) {
-    case AttemptState_AttemptState: {
-      data2, ok := other.Get_().(AttemptState_AttemptState)
-      return ok && data1.Phase.Equals(data2.Phase) && data1.RecoveryDispatches.Cmp(data2.RecoveryDispatches) == 0 && data1.DispatchedEffects.Equals(data2.DispatchedEffects) && data1.ProcessedCmdKeys.Equals(data2.ProcessedCmdKeys) && data1.Version.Cmp(data2.Version) == 0
-    }
-    default: {
-      return false; // unexpected
-    }
-  }
+	switch data1 := _this.Get_().(type) {
+	case AttemptState_AttemptState:
+		{
+			data2, ok := other.Get_().(AttemptState_AttemptState)
+			return ok && data1.Phase.Equals(data2.Phase) && data1.RecoveryDispatches.Cmp(data2.RecoveryDispatches) == 0 && data1.DispatchedEffects.Equals(data2.DispatchedEffects) && data1.ProcessedCmdKeys.Equals(data2.ProcessedCmdKeys) && data1.Version.Cmp(data2.Version) == 0
+		}
+	default:
+		{
+			return false // unexpected
+		}
+	}
 }
 
 func (_this AttemptState) EqualsGeneric(other interface{}) bool {
-  typed, ok := other.(AttemptState)
-  return ok && _this.Equals(typed)
+	typed, ok := other.(AttemptState)
+	return ok && _this.Equals(typed)
 }
 
 func Type_AttemptState_() _dafny.TypeDescriptor {
-  return type_AttemptState_{}
+	return type_AttemptState_{}
 }
 
 type type_AttemptState_ struct {
 }
 
 func (_this type_AttemptState_) Default() interface{} {
-  return Companion_AttemptState_.Default();
+	return Companion_AttemptState_.Default()
 }
 
 func (_this type_AttemptState_) String() string {
-  return "Reducer.AttemptState"
+	return "Reducer.AttemptState"
 }
 func (_this AttemptState) ParentTraits_() []*_dafny.TraitID {
-  return [](*_dafny.TraitID){};
+	return [](*_dafny.TraitID){}
 }
+
 var _ _dafny.TraitOffspring = AttemptState{}
 
 // End of datatype AttemptState
 
 // Definition of datatype Command
 type Command struct {
-  Data_Command_
+	Data_Command_
 }
 
 func (_this Command) Get_() Data_Command_ {
-  return _this.Data_Command_
+	return _this.Data_Command_
 }
 
 type Data_Command_ interface {
-  isCommand()
+	isCommand()
 }
 
 type CompanionStruct_Command_ struct {
 }
-var Companion_Command_ = CompanionStruct_Command_ {
-}
+
+var Companion_Command_ = CompanionStruct_Command_{}
 
 type Command_CommandProposeRecovery struct {
-  AttemptID _dafny.Sequence
-  IdempotencyKey _dafny.Sequence
-  Version _dafny.Int
+	AttemptID      _dafny.Sequence
+	IdempotencyKey _dafny.Sequence
+	Version        _dafny.Int
 }
 
 func (Command_CommandProposeRecovery) isCommand() {}
 
 func (CompanionStruct_Command_) Create_CommandProposeRecovery_(AttemptID _dafny.Sequence, IdempotencyKey _dafny.Sequence, Version _dafny.Int) Command {
-  return Command{Command_CommandProposeRecovery{AttemptID, IdempotencyKey, Version}}
+	return Command{Command_CommandProposeRecovery{AttemptID, IdempotencyKey, Version}}
 }
 
 func (_this Command) Is_CommandProposeRecovery() bool {
-  _, ok := _this.Get_().(Command_CommandProposeRecovery)
-  return ok
+	_, ok := _this.Get_().(Command_CommandProposeRecovery)
+	return ok
 }
 
 type Command_CommandConclude struct {
-  AttemptID _dafny.Sequence
+	AttemptID _dafny.Sequence
 }
 
 func (Command_CommandConclude) isCommand() {}
 
 func (CompanionStruct_Command_) Create_CommandConclude_(AttemptID _dafny.Sequence) Command {
-  return Command{Command_CommandConclude{AttemptID}}
+	return Command{Command_CommandConclude{AttemptID}}
 }
 
 func (_this Command) Is_CommandConclude() bool {
-  _, ok := _this.Get_().(Command_CommandConclude)
-  return ok
+	_, ok := _this.Get_().(Command_CommandConclude)
+	return ok
 }
 
 type Command_CommandUnknown struct {
-  AttemptID _dafny.Sequence
+	AttemptID _dafny.Sequence
 }
 
 func (Command_CommandUnknown) isCommand() {}
 
 func (CompanionStruct_Command_) Create_CommandUnknown_(AttemptID _dafny.Sequence) Command {
-  return Command{Command_CommandUnknown{AttemptID}}
+	return Command{Command_CommandUnknown{AttemptID}}
 }
 
 func (_this Command) Is_CommandUnknown() bool {
-  _, ok := _this.Get_().(Command_CommandUnknown)
-  return ok
+	_, ok := _this.Get_().(Command_CommandUnknown)
+	return ok
 }
 
 func (CompanionStruct_Command_) Default() Command {
-  return Companion_Command_.Create_CommandProposeRecovery_(_dafny.EmptySeq, _dafny.EmptySeq, _dafny.Zero)
+	return Companion_Command_.Create_CommandProposeRecovery_(_dafny.EmptySeq, _dafny.EmptySeq, _dafny.Zero)
 }
 
 func (_this Command) Dtor_attemptID() _dafny.Sequence {
-  switch data := _this.Get_().(type) {
-    case Command_CommandProposeRecovery: return data.AttemptID
-    case Command_CommandConclude: return data.AttemptID
-    default: return data.(Command_CommandUnknown).AttemptID
-  }
+	switch data := _this.Get_().(type) {
+	case Command_CommandProposeRecovery:
+		return data.AttemptID
+	case Command_CommandConclude:
+		return data.AttemptID
+	default:
+		return data.(Command_CommandUnknown).AttemptID
+	}
 }
 
 func (_this Command) Dtor_idempotencyKey() _dafny.Sequence {
-  return _this.Get_().(Command_CommandProposeRecovery).IdempotencyKey
+	return _this.Get_().(Command_CommandProposeRecovery).IdempotencyKey
 }
 
 func (_this Command) Dtor_version() _dafny.Int {
-  return _this.Get_().(Command_CommandProposeRecovery).Version
+	return _this.Get_().(Command_CommandProposeRecovery).Version
 }
 
 func (_this Command) String() string {
-  switch data := _this.Get_().(type) {
-    case nil: return "null"
-    case Command_CommandProposeRecovery: {
-      return "Reducer.Command.CommandProposeRecovery" + "(" + data.AttemptID.VerbatimString(true) + ", " + data.IdempotencyKey.VerbatimString(true) + ", " + _dafny.String(data.Version) + ")"
-    }
-    case Command_CommandConclude: {
-      return "Reducer.Command.CommandConclude" + "(" + data.AttemptID.VerbatimString(true) + ")"
-    }
-    case Command_CommandUnknown: {
-      return "Reducer.Command.CommandUnknown" + "(" + data.AttemptID.VerbatimString(true) + ")"
-    }
-    default: {
-      return "<unexpected>"
-    }
-  }
+	switch data := _this.Get_().(type) {
+	case nil:
+		return "null"
+	case Command_CommandProposeRecovery:
+		{
+			return "Reducer.Command.CommandProposeRecovery" + "(" + data.AttemptID.VerbatimString(true) + ", " + data.IdempotencyKey.VerbatimString(true) + ", " + _dafny.String(data.Version) + ")"
+		}
+	case Command_CommandConclude:
+		{
+			return "Reducer.Command.CommandConclude" + "(" + data.AttemptID.VerbatimString(true) + ")"
+		}
+	case Command_CommandUnknown:
+		{
+			return "Reducer.Command.CommandUnknown" + "(" + data.AttemptID.VerbatimString(true) + ")"
+		}
+	default:
+		{
+			return "<unexpected>"
+		}
+	}
 }
 
 func (_this Command) Equals(other Command) bool {
-  switch data1 := _this.Get_().(type) {
-    case Command_CommandProposeRecovery: {
-      data2, ok := other.Get_().(Command_CommandProposeRecovery)
-      return ok && data1.AttemptID.Equals(data2.AttemptID) && data1.IdempotencyKey.Equals(data2.IdempotencyKey) && data1.Version.Cmp(data2.Version) == 0
-    }
-    case Command_CommandConclude: {
-      data2, ok := other.Get_().(Command_CommandConclude)
-      return ok && data1.AttemptID.Equals(data2.AttemptID)
-    }
-    case Command_CommandUnknown: {
-      data2, ok := other.Get_().(Command_CommandUnknown)
-      return ok && data1.AttemptID.Equals(data2.AttemptID)
-    }
-    default: {
-      return false; // unexpected
-    }
-  }
+	switch data1 := _this.Get_().(type) {
+	case Command_CommandProposeRecovery:
+		{
+			data2, ok := other.Get_().(Command_CommandProposeRecovery)
+			return ok && data1.AttemptID.Equals(data2.AttemptID) && data1.IdempotencyKey.Equals(data2.IdempotencyKey) && data1.Version.Cmp(data2.Version) == 0
+		}
+	case Command_CommandConclude:
+		{
+			data2, ok := other.Get_().(Command_CommandConclude)
+			return ok && data1.AttemptID.Equals(data2.AttemptID)
+		}
+	case Command_CommandUnknown:
+		{
+			data2, ok := other.Get_().(Command_CommandUnknown)
+			return ok && data1.AttemptID.Equals(data2.AttemptID)
+		}
+	default:
+		{
+			return false // unexpected
+		}
+	}
 }
 
 func (_this Command) EqualsGeneric(other interface{}) bool {
-  typed, ok := other.(Command)
-  return ok && _this.Equals(typed)
+	typed, ok := other.(Command)
+	return ok && _this.Equals(typed)
 }
 
 func Type_Command_() _dafny.TypeDescriptor {
-  return type_Command_{}
+	return type_Command_{}
 }
 
 type type_Command_ struct {
 }
 
 func (_this type_Command_) Default() interface{} {
-  return Companion_Command_.Default();
+	return Companion_Command_.Default()
 }
 
 func (_this type_Command_) String() string {
-  return "Reducer.Command"
+	return "Reducer.Command"
 }
 func (_this Command) ParentTraits_() []*_dafny.TraitID {
-  return [](*_dafny.TraitID){};
+	return [](*_dafny.TraitID){}
 }
+
 var _ _dafny.TraitOffspring = Command{}
 
 // End of datatype Command
 
 // Definition of datatype Event
 type Event struct {
-  Data_Event_
+	Data_Event_
 }
 
 func (_this Event) Get_() Data_Event_ {
-  return _this.Data_Event_
+	return _this.Data_Event_
 }
 
 type Data_Event_ interface {
-  isEvent()
+	isEvent()
 }
 
 type CompanionStruct_Event_ struct {
 }
-var Companion_Event_ = CompanionStruct_Event_ {
-}
+
+var Companion_Event_ = CompanionStruct_Event_{}
 
 type Event_EventRecoveryDispatched struct {
-  AttemptID _dafny.Sequence
-  EffectID _dafny.Sequence
-  Ordinal _dafny.Int
-  IdempotencyKey _dafny.Sequence
+	AttemptID      _dafny.Sequence
+	EffectID       _dafny.Sequence
+	Ordinal        _dafny.Int
+	IdempotencyKey _dafny.Sequence
 }
 
 func (Event_EventRecoveryDispatched) isEvent() {}
 
 func (CompanionStruct_Event_) Create_EventRecoveryDispatched_(AttemptID _dafny.Sequence, EffectID _dafny.Sequence, Ordinal _dafny.Int, IdempotencyKey _dafny.Sequence) Event {
-  return Event{Event_EventRecoveryDispatched{AttemptID, EffectID, Ordinal, IdempotencyKey}}
+	return Event{Event_EventRecoveryDispatched{AttemptID, EffectID, Ordinal, IdempotencyKey}}
 }
 
 func (_this Event) Is_EventRecoveryDispatched() bool {
-  _, ok := _this.Get_().(Event_EventRecoveryDispatched)
-  return ok
+	_, ok := _this.Get_().(Event_EventRecoveryDispatched)
+	return ok
 }
 
 type Event_EventRecoveryRejected struct {
-  AttemptID _dafny.Sequence
-  Reason _dafny.Sequence
+	AttemptID _dafny.Sequence
+	Reason    _dafny.Sequence
 }
 
 func (Event_EventRecoveryRejected) isEvent() {}
 
 func (CompanionStruct_Event_) Create_EventRecoveryRejected_(AttemptID _dafny.Sequence, Reason _dafny.Sequence) Event {
-  return Event{Event_EventRecoveryRejected{AttemptID, Reason}}
+	return Event{Event_EventRecoveryRejected{AttemptID, Reason}}
 }
 
 func (_this Event) Is_EventRecoveryRejected() bool {
-  _, ok := _this.Get_().(Event_EventRecoveryRejected)
-  return ok
+	_, ok := _this.Get_().(Event_EventRecoveryRejected)
+	return ok
 }
 
 type Event_EventConcluded struct {
-  AttemptID _dafny.Sequence
+	AttemptID _dafny.Sequence
 }
 
 func (Event_EventConcluded) isEvent() {}
 
 func (CompanionStruct_Event_) Create_EventConcluded_(AttemptID _dafny.Sequence) Event {
-  return Event{Event_EventConcluded{AttemptID}}
+	return Event{Event_EventConcluded{AttemptID}}
 }
 
 func (_this Event) Is_EventConcluded() bool {
-  _, ok := _this.Get_().(Event_EventConcluded)
-  return ok
+	_, ok := _this.Get_().(Event_EventConcluded)
+	return ok
 }
 
 func (CompanionStruct_Event_) Default() Event {
-  return Companion_Event_.Create_EventRecoveryDispatched_(_dafny.EmptySeq, _dafny.EmptySeq, _dafny.Zero, _dafny.EmptySeq)
+	return Companion_Event_.Create_EventRecoveryDispatched_(_dafny.EmptySeq, _dafny.EmptySeq, _dafny.Zero, _dafny.EmptySeq)
 }
 
 func (_this Event) Dtor_attemptID() _dafny.Sequence {
-  switch data := _this.Get_().(type) {
-    case Event_EventRecoveryDispatched: return data.AttemptID
-    case Event_EventRecoveryRejected: return data.AttemptID
-    default: return data.(Event_EventConcluded).AttemptID
-  }
+	switch data := _this.Get_().(type) {
+	case Event_EventRecoveryDispatched:
+		return data.AttemptID
+	case Event_EventRecoveryRejected:
+		return data.AttemptID
+	default:
+		return data.(Event_EventConcluded).AttemptID
+	}
 }
 
 func (_this Event) Dtor_effectID() _dafny.Sequence {
-  return _this.Get_().(Event_EventRecoveryDispatched).EffectID
+	return _this.Get_().(Event_EventRecoveryDispatched).EffectID
 }
 
 func (_this Event) Dtor_ordinal() _dafny.Int {
-  return _this.Get_().(Event_EventRecoveryDispatched).Ordinal
+	return _this.Get_().(Event_EventRecoveryDispatched).Ordinal
 }
 
 func (_this Event) Dtor_idempotencyKey() _dafny.Sequence {
-  return _this.Get_().(Event_EventRecoveryDispatched).IdempotencyKey
+	return _this.Get_().(Event_EventRecoveryDispatched).IdempotencyKey
 }
 
 func (_this Event) Dtor_reason() _dafny.Sequence {
-  return _this.Get_().(Event_EventRecoveryRejected).Reason
+	return _this.Get_().(Event_EventRecoveryRejected).Reason
 }
 
 func (_this Event) String() string {
-  switch data := _this.Get_().(type) {
-    case nil: return "null"
-    case Event_EventRecoveryDispatched: {
-      return "Reducer.Event.EventRecoveryDispatched" + "(" + data.AttemptID.VerbatimString(true) + ", " + data.EffectID.VerbatimString(true) + ", " + _dafny.String(data.Ordinal) + ", " + data.IdempotencyKey.VerbatimString(true) + ")"
-    }
-    case Event_EventRecoveryRejected: {
-      return "Reducer.Event.EventRecoveryRejected" + "(" + data.AttemptID.VerbatimString(true) + ", " + data.Reason.VerbatimString(true) + ")"
-    }
-    case Event_EventConcluded: {
-      return "Reducer.Event.EventConcluded" + "(" + data.AttemptID.VerbatimString(true) + ")"
-    }
-    default: {
-      return "<unexpected>"
-    }
-  }
+	switch data := _this.Get_().(type) {
+	case nil:
+		return "null"
+	case Event_EventRecoveryDispatched:
+		{
+			return "Reducer.Event.EventRecoveryDispatched" + "(" + data.AttemptID.VerbatimString(true) + ", " + data.EffectID.VerbatimString(true) + ", " + _dafny.String(data.Ordinal) + ", " + data.IdempotencyKey.VerbatimString(true) + ")"
+		}
+	case Event_EventRecoveryRejected:
+		{
+			return "Reducer.Event.EventRecoveryRejected" + "(" + data.AttemptID.VerbatimString(true) + ", " + data.Reason.VerbatimString(true) + ")"
+		}
+	case Event_EventConcluded:
+		{
+			return "Reducer.Event.EventConcluded" + "(" + data.AttemptID.VerbatimString(true) + ")"
+		}
+	default:
+		{
+			return "<unexpected>"
+		}
+	}
 }
 
 func (_this Event) Equals(other Event) bool {
-  switch data1 := _this.Get_().(type) {
-    case Event_EventRecoveryDispatched: {
-      data2, ok := other.Get_().(Event_EventRecoveryDispatched)
-      return ok && data1.AttemptID.Equals(data2.AttemptID) && data1.EffectID.Equals(data2.EffectID) && data1.Ordinal.Cmp(data2.Ordinal) == 0 && data1.IdempotencyKey.Equals(data2.IdempotencyKey)
-    }
-    case Event_EventRecoveryRejected: {
-      data2, ok := other.Get_().(Event_EventRecoveryRejected)
-      return ok && data1.AttemptID.Equals(data2.AttemptID) && data1.Reason.Equals(data2.Reason)
-    }
-    case Event_EventConcluded: {
-      data2, ok := other.Get_().(Event_EventConcluded)
-      return ok && data1.AttemptID.Equals(data2.AttemptID)
-    }
-    default: {
-      return false; // unexpected
-    }
-  }
+	switch data1 := _this.Get_().(type) {
+	case Event_EventRecoveryDispatched:
+		{
+			data2, ok := other.Get_().(Event_EventRecoveryDispatched)
+			return ok && data1.AttemptID.Equals(data2.AttemptID) && data1.EffectID.Equals(data2.EffectID) && data1.Ordinal.Cmp(data2.Ordinal) == 0 && data1.IdempotencyKey.Equals(data2.IdempotencyKey)
+		}
+	case Event_EventRecoveryRejected:
+		{
+			data2, ok := other.Get_().(Event_EventRecoveryRejected)
+			return ok && data1.AttemptID.Equals(data2.AttemptID) && data1.Reason.Equals(data2.Reason)
+		}
+	case Event_EventConcluded:
+		{
+			data2, ok := other.Get_().(Event_EventConcluded)
+			return ok && data1.AttemptID.Equals(data2.AttemptID)
+		}
+	default:
+		{
+			return false // unexpected
+		}
+	}
 }
 
 func (_this Event) EqualsGeneric(other interface{}) bool {
-  typed, ok := other.(Event)
-  return ok && _this.Equals(typed)
+	typed, ok := other.(Event)
+	return ok && _this.Equals(typed)
 }
 
 func Type_Event_() _dafny.TypeDescriptor {
-  return type_Event_{}
+	return type_Event_{}
 }
 
 type type_Event_ struct {
 }
 
 func (_this type_Event_) Default() interface{} {
-  return Companion_Event_.Default();
+	return Companion_Event_.Default()
 }
 
 func (_this type_Event_) String() string {
-  return "Reducer.Event"
+	return "Reducer.Event"
 }
 func (_this Event) ParentTraits_() []*_dafny.TraitID {
-  return [](*_dafny.TraitID){};
+	return [](*_dafny.TraitID){}
 }
+
 var _ _dafny.TraitOffspring = Event{}
 
 // End of datatype Event
 
 // Definition of datatype EffectIntent
 type EffectIntent struct {
-  Data_EffectIntent_
+	Data_EffectIntent_
 }
 
 func (_this EffectIntent) Get_() Data_EffectIntent_ {
-  return _this.Data_EffectIntent_
+	return _this.Data_EffectIntent_
 }
 
 type Data_EffectIntent_ interface {
-  isEffectIntent()
+	isEffectIntent()
 }
 
 type CompanionStruct_EffectIntent_ struct {
 }
-var Companion_EffectIntent_ = CompanionStruct_EffectIntent_ {
-}
+
+var Companion_EffectIntent_ = CompanionStruct_EffectIntent_{}
 
 type EffectIntent_EffectIntent struct {
-  AttemptID _dafny.Sequence
-  EffectID _dafny.Sequence
-  Ordinal _dafny.Int
+	AttemptID _dafny.Sequence
+	EffectID  _dafny.Sequence
+	Ordinal   _dafny.Int
 }
 
 func (EffectIntent_EffectIntent) isEffectIntent() {}
 
 func (CompanionStruct_EffectIntent_) Create_EffectIntent_(AttemptID _dafny.Sequence, EffectID _dafny.Sequence, Ordinal _dafny.Int) EffectIntent {
-  return EffectIntent{EffectIntent_EffectIntent{AttemptID, EffectID, Ordinal}}
+	return EffectIntent{EffectIntent_EffectIntent{AttemptID, EffectID, Ordinal}}
 }
 
 func (_this EffectIntent) Is_EffectIntent() bool {
-  _, ok := _this.Get_().(EffectIntent_EffectIntent)
-  return ok
+	_, ok := _this.Get_().(EffectIntent_EffectIntent)
+	return ok
 }
 
 func (CompanionStruct_EffectIntent_) Default() EffectIntent {
-  return Companion_EffectIntent_.Create_EffectIntent_(_dafny.EmptySeq, _dafny.EmptySeq, _dafny.Zero)
+	return Companion_EffectIntent_.Create_EffectIntent_(_dafny.EmptySeq, _dafny.EmptySeq, _dafny.Zero)
 }
 
 func (_this EffectIntent) Dtor_attemptID() _dafny.Sequence {
-  return _this.Get_().(EffectIntent_EffectIntent).AttemptID
+	return _this.Get_().(EffectIntent_EffectIntent).AttemptID
 }
 
 func (_this EffectIntent) Dtor_effectID() _dafny.Sequence {
-  return _this.Get_().(EffectIntent_EffectIntent).EffectID
+	return _this.Get_().(EffectIntent_EffectIntent).EffectID
 }
 
 func (_this EffectIntent) Dtor_ordinal() _dafny.Int {
-  return _this.Get_().(EffectIntent_EffectIntent).Ordinal
+	return _this.Get_().(EffectIntent_EffectIntent).Ordinal
 }
 
 func (_this EffectIntent) String() string {
-  switch data := _this.Get_().(type) {
-    case nil: return "null"
-    case EffectIntent_EffectIntent: {
-      return "Reducer.EffectIntent.EffectIntent" + "(" + data.AttemptID.VerbatimString(true) + ", " + data.EffectID.VerbatimString(true) + ", " + _dafny.String(data.Ordinal) + ")"
-    }
-    default: {
-      return "<unexpected>"
-    }
-  }
+	switch data := _this.Get_().(type) {
+	case nil:
+		return "null"
+	case EffectIntent_EffectIntent:
+		{
+			return "Reducer.EffectIntent.EffectIntent" + "(" + data.AttemptID.VerbatimString(true) + ", " + data.EffectID.VerbatimString(true) + ", " + _dafny.String(data.Ordinal) + ")"
+		}
+	default:
+		{
+			return "<unexpected>"
+		}
+	}
 }
 
 func (_this EffectIntent) Equals(other EffectIntent) bool {
-  switch data1 := _this.Get_().(type) {
-    case EffectIntent_EffectIntent: {
-      data2, ok := other.Get_().(EffectIntent_EffectIntent)
-      return ok && data1.AttemptID.Equals(data2.AttemptID) && data1.EffectID.Equals(data2.EffectID) && data1.Ordinal.Cmp(data2.Ordinal) == 0
-    }
-    default: {
-      return false; // unexpected
-    }
-  }
+	switch data1 := _this.Get_().(type) {
+	case EffectIntent_EffectIntent:
+		{
+			data2, ok := other.Get_().(EffectIntent_EffectIntent)
+			return ok && data1.AttemptID.Equals(data2.AttemptID) && data1.EffectID.Equals(data2.EffectID) && data1.Ordinal.Cmp(data2.Ordinal) == 0
+		}
+	default:
+		{
+			return false // unexpected
+		}
+	}
 }
 
 func (_this EffectIntent) EqualsGeneric(other interface{}) bool {
-  typed, ok := other.(EffectIntent)
-  return ok && _this.Equals(typed)
+	typed, ok := other.(EffectIntent)
+	return ok && _this.Equals(typed)
 }
 
 func Type_EffectIntent_() _dafny.TypeDescriptor {
-  return type_EffectIntent_{}
+	return type_EffectIntent_{}
 }
 
 type type_EffectIntent_ struct {
 }
 
 func (_this type_EffectIntent_) Default() interface{} {
-  return Companion_EffectIntent_.Default();
+	return Companion_EffectIntent_.Default()
 }
 
 func (_this type_EffectIntent_) String() string {
-  return "Reducer.EffectIntent"
+	return "Reducer.EffectIntent"
 }
 func (_this EffectIntent) ParentTraits_() []*_dafny.TraitID {
-  return [](*_dafny.TraitID){};
+	return [](*_dafny.TraitID){}
 }
+
 var _ _dafny.TraitOffspring = EffectIntent{}
 
 // End of datatype EffectIntent
 
 // Definition of datatype DecisionStatus
 type DecisionStatus struct {
-  Data_DecisionStatus_
+	Data_DecisionStatus_
 }
 
 func (_this DecisionStatus) Get_() Data_DecisionStatus_ {
-  return _this.Data_DecisionStatus_
+	return _this.Data_DecisionStatus_
 }
 
 type Data_DecisionStatus_ interface {
-  isDecisionStatus()
+	isDecisionStatus()
 }
 
 type CompanionStruct_DecisionStatus_ struct {
 }
-var Companion_DecisionStatus_ = CompanionStruct_DecisionStatus_ {
-}
+
+var Companion_DecisionStatus_ = CompanionStruct_DecisionStatus_{}
 
 type DecisionStatus_Accepted struct {
 }
@@ -818,12 +872,12 @@ type DecisionStatus_Accepted struct {
 func (DecisionStatus_Accepted) isDecisionStatus() {}
 
 func (CompanionStruct_DecisionStatus_) Create_Accepted_() DecisionStatus {
-  return DecisionStatus{DecisionStatus_Accepted{}}
+	return DecisionStatus{DecisionStatus_Accepted{}}
 }
 
 func (_this DecisionStatus) Is_Accepted() bool {
-  _, ok := _this.Get_().(DecisionStatus_Accepted)
-  return ok
+	_, ok := _this.Get_().(DecisionStatus_Accepted)
+	return ok
 }
 
 type DecisionStatus_Rejected struct {
@@ -832,12 +886,12 @@ type DecisionStatus_Rejected struct {
 func (DecisionStatus_Rejected) isDecisionStatus() {}
 
 func (CompanionStruct_DecisionStatus_) Create_Rejected_() DecisionStatus {
-  return DecisionStatus{DecisionStatus_Rejected{}}
+	return DecisionStatus{DecisionStatus_Rejected{}}
 }
 
 func (_this DecisionStatus) Is_Rejected() bool {
-  _, ok := _this.Get_().(DecisionStatus_Rejected)
-  return ok
+	_, ok := _this.Get_().(DecisionStatus_Rejected)
+	return ok
 }
 
 type DecisionStatus_NoOp struct {
@@ -846,192 +900,212 @@ type DecisionStatus_NoOp struct {
 func (DecisionStatus_NoOp) isDecisionStatus() {}
 
 func (CompanionStruct_DecisionStatus_) Create_NoOp_() DecisionStatus {
-  return DecisionStatus{DecisionStatus_NoOp{}}
+	return DecisionStatus{DecisionStatus_NoOp{}}
 }
 
 func (_this DecisionStatus) Is_NoOp() bool {
-  _, ok := _this.Get_().(DecisionStatus_NoOp)
-  return ok
+	_, ok := _this.Get_().(DecisionStatus_NoOp)
+	return ok
 }
 
 func (CompanionStruct_DecisionStatus_) Default() DecisionStatus {
-  return Companion_DecisionStatus_.Create_Accepted_()
+	return Companion_DecisionStatus_.Create_Accepted_()
 }
 
 func (_ CompanionStruct_DecisionStatus_) AllSingletonConstructors() _dafny.Iterator {
-  i := -1
-  return func() (interface{}, bool) {
-    i++
-    switch i {
-      case 0: return Companion_DecisionStatus_.Create_Accepted_(), true
-      case 1: return Companion_DecisionStatus_.Create_Rejected_(), true
-      case 2: return Companion_DecisionStatus_.Create_NoOp_(), true
-      default: return DecisionStatus{}, false
-    }
-  }
+	i := -1
+	return func() (interface{}, bool) {
+		i++
+		switch i {
+		case 0:
+			return Companion_DecisionStatus_.Create_Accepted_(), true
+		case 1:
+			return Companion_DecisionStatus_.Create_Rejected_(), true
+		case 2:
+			return Companion_DecisionStatus_.Create_NoOp_(), true
+		default:
+			return DecisionStatus{}, false
+		}
+	}
 }
 
 func (_this DecisionStatus) String() string {
-  switch _this.Get_().(type) {
-    case nil: return "null"
-    case DecisionStatus_Accepted: {
-      return "Reducer.DecisionStatus.Accepted"
-    }
-    case DecisionStatus_Rejected: {
-      return "Reducer.DecisionStatus.Rejected"
-    }
-    case DecisionStatus_NoOp: {
-      return "Reducer.DecisionStatus.NoOp"
-    }
-    default: {
-      return "<unexpected>"
-    }
-  }
+	switch _this.Get_().(type) {
+	case nil:
+		return "null"
+	case DecisionStatus_Accepted:
+		{
+			return "Reducer.DecisionStatus.Accepted"
+		}
+	case DecisionStatus_Rejected:
+		{
+			return "Reducer.DecisionStatus.Rejected"
+		}
+	case DecisionStatus_NoOp:
+		{
+			return "Reducer.DecisionStatus.NoOp"
+		}
+	default:
+		{
+			return "<unexpected>"
+		}
+	}
 }
 
 func (_this DecisionStatus) Equals(other DecisionStatus) bool {
-  switch _this.Get_().(type) {
-    case DecisionStatus_Accepted: {
-      _, ok := other.Get_().(DecisionStatus_Accepted)
-      return ok
-    }
-    case DecisionStatus_Rejected: {
-      _, ok := other.Get_().(DecisionStatus_Rejected)
-      return ok
-    }
-    case DecisionStatus_NoOp: {
-      _, ok := other.Get_().(DecisionStatus_NoOp)
-      return ok
-    }
-    default: {
-      return false; // unexpected
-    }
-  }
+	switch _this.Get_().(type) {
+	case DecisionStatus_Accepted:
+		{
+			_, ok := other.Get_().(DecisionStatus_Accepted)
+			return ok
+		}
+	case DecisionStatus_Rejected:
+		{
+			_, ok := other.Get_().(DecisionStatus_Rejected)
+			return ok
+		}
+	case DecisionStatus_NoOp:
+		{
+			_, ok := other.Get_().(DecisionStatus_NoOp)
+			return ok
+		}
+	default:
+		{
+			return false // unexpected
+		}
+	}
 }
 
 func (_this DecisionStatus) EqualsGeneric(other interface{}) bool {
-  typed, ok := other.(DecisionStatus)
-  return ok && _this.Equals(typed)
+	typed, ok := other.(DecisionStatus)
+	return ok && _this.Equals(typed)
 }
 
 func Type_DecisionStatus_() _dafny.TypeDescriptor {
-  return type_DecisionStatus_{}
+	return type_DecisionStatus_{}
 }
 
 type type_DecisionStatus_ struct {
 }
 
 func (_this type_DecisionStatus_) Default() interface{} {
-  return Companion_DecisionStatus_.Default();
+	return Companion_DecisionStatus_.Default()
 }
 
 func (_this type_DecisionStatus_) String() string {
-  return "Reducer.DecisionStatus"
+	return "Reducer.DecisionStatus"
 }
 func (_this DecisionStatus) ParentTraits_() []*_dafny.TraitID {
-  return [](*_dafny.TraitID){};
+	return [](*_dafny.TraitID){}
 }
+
 var _ _dafny.TraitOffspring = DecisionStatus{}
 
 // End of datatype DecisionStatus
 
 // Definition of datatype Decision
 type Decision struct {
-  Data_Decision_
+	Data_Decision_
 }
 
 func (_this Decision) Get_() Data_Decision_ {
-  return _this.Data_Decision_
+	return _this.Data_Decision_
 }
 
 type Data_Decision_ interface {
-  isDecision()
+	isDecision()
 }
 
 type CompanionStruct_Decision_ struct {
 }
-var Companion_Decision_ = CompanionStruct_Decision_ {
-}
+
+var Companion_Decision_ = CompanionStruct_Decision_{}
 
 type Decision_Decision struct {
-  Status DecisionStatus
-  Events _dafny.Sequence
-  Effects _dafny.Sequence
+	Status  DecisionStatus
+	Events  _dafny.Sequence
+	Effects _dafny.Sequence
 }
 
 func (Decision_Decision) isDecision() {}
 
 func (CompanionStruct_Decision_) Create_Decision_(Status DecisionStatus, Events _dafny.Sequence, Effects _dafny.Sequence) Decision {
-  return Decision{Decision_Decision{Status, Events, Effects}}
+	return Decision{Decision_Decision{Status, Events, Effects}}
 }
 
 func (_this Decision) Is_Decision() bool {
-  _, ok := _this.Get_().(Decision_Decision)
-  return ok
+	_, ok := _this.Get_().(Decision_Decision)
+	return ok
 }
 
 func (CompanionStruct_Decision_) Default() Decision {
-  return Companion_Decision_.Create_Decision_(Companion_DecisionStatus_.Default(), _dafny.EmptySeq, _dafny.EmptySeq)
+	return Companion_Decision_.Create_Decision_(Companion_DecisionStatus_.Default(), _dafny.EmptySeq, _dafny.EmptySeq)
 }
 
 func (_this Decision) Dtor_status() DecisionStatus {
-  return _this.Get_().(Decision_Decision).Status
+	return _this.Get_().(Decision_Decision).Status
 }
 
 func (_this Decision) Dtor_events() _dafny.Sequence {
-  return _this.Get_().(Decision_Decision).Events
+	return _this.Get_().(Decision_Decision).Events
 }
 
 func (_this Decision) Dtor_effects() _dafny.Sequence {
-  return _this.Get_().(Decision_Decision).Effects
+	return _this.Get_().(Decision_Decision).Effects
 }
 
 func (_this Decision) String() string {
-  switch data := _this.Get_().(type) {
-    case nil: return "null"
-    case Decision_Decision: {
-      return "Reducer.Decision.Decision" + "(" + _dafny.String(data.Status) + ", " + _dafny.String(data.Events) + ", " + _dafny.String(data.Effects) + ")"
-    }
-    default: {
-      return "<unexpected>"
-    }
-  }
+	switch data := _this.Get_().(type) {
+	case nil:
+		return "null"
+	case Decision_Decision:
+		{
+			return "Reducer.Decision.Decision" + "(" + _dafny.String(data.Status) + ", " + _dafny.String(data.Events) + ", " + _dafny.String(data.Effects) + ")"
+		}
+	default:
+		{
+			return "<unexpected>"
+		}
+	}
 }
 
 func (_this Decision) Equals(other Decision) bool {
-  switch data1 := _this.Get_().(type) {
-    case Decision_Decision: {
-      data2, ok := other.Get_().(Decision_Decision)
-      return ok && data1.Status.Equals(data2.Status) && data1.Events.Equals(data2.Events) && data1.Effects.Equals(data2.Effects)
-    }
-    default: {
-      return false; // unexpected
-    }
-  }
+	switch data1 := _this.Get_().(type) {
+	case Decision_Decision:
+		{
+			data2, ok := other.Get_().(Decision_Decision)
+			return ok && data1.Status.Equals(data2.Status) && data1.Events.Equals(data2.Events) && data1.Effects.Equals(data2.Effects)
+		}
+	default:
+		{
+			return false // unexpected
+		}
+	}
 }
 
 func (_this Decision) EqualsGeneric(other interface{}) bool {
-  typed, ok := other.(Decision)
-  return ok && _this.Equals(typed)
+	typed, ok := other.(Decision)
+	return ok && _this.Equals(typed)
 }
 
 func Type_Decision_() _dafny.TypeDescriptor {
-  return type_Decision_{}
+	return type_Decision_{}
 }
 
 type type_Decision_ struct {
 }
 
 func (_this type_Decision_) Default() interface{} {
-  return Companion_Decision_.Default();
+	return Companion_Decision_.Default()
 }
 
 func (_this type_Decision_) String() string {
-  return "Reducer.Decision"
+	return "Reducer.Decision"
 }
 func (_this Decision) ParentTraits_() []*_dafny.TraitID {
-  return [](*_dafny.TraitID){};
+	return [](*_dafny.TraitID){}
 }
+
 var _ _dafny.TraitOffspring = Decision{}
 
 // End of datatype Decision
